Update standard benchmarks

benchmarks/standard/tree/common.v
@@ -8,6 +8,7 @@ From SSL
 Require Import core.
 From Hammer Require Import Hammer.
 (* Configure Hammer *)
+Set Hammer ATPLimit 60.
 Unset Hammer Eprover.
 Unset Hammer Vampire.
 Add Search Blacklist "fcsl.".
@@ -28,8 +29,8 @@ Inductive sll (x : ptr) (s : seq nat) (h : heap) : Prop :=
   (s) == (@nil nat) /\ h = empty
 | sll_2 of ~~ ((x) == (null)) of
   exists (v : nat) (s1 : seq nat) (nxt : ptr),
-  exists h_sll_nxts1_543,
-  (s) == (([:: v]) ++ (s1)) /\ h = x :-> v \+ x .+ 1 :-> nxt \+ h_sll_nxts1_543 /\ sll nxt s1 h_sll_nxts1_543.
+  exists h_sll_nxts1_4,
+  (s) == (([:: v]) ++ (s1)) /\ h = x :-> (v) \+ x .+ 1 :-> (nxt) \+ h_sll_nxts1_4 /\ sll nxt s1 h_sll_nxts1_4.
 
 
 Inductive treeN (x : ptr) (n : nat) (h : heap) : Prop :=
@@ -37,8 +38,8 @@ Inductive treeN (x : ptr) (n : nat) (h : heap) : Prop :=
   (n) == (0) /\ h = empty
 | treeN_2 of ~~ ((x) == (null)) of
   exists (n1 : nat) (n2 : nat) (l : ptr) (r : ptr) (v : ptr),
-  exists h_treeN_ln1_541 h_treeN_rn2_542,
-  (0) <= (n1) /\ (0) <= (n2) /\ (n) == (((1) + (n1)) + (n2)) /\ h = x :-> v \+ x .+ 1 :-> l \+ x .+ 2 :-> r \+ h_treeN_ln1_541 \+ h_treeN_rn2_542 /\ treeN l n1 h_treeN_ln1_541 /\ treeN r n2 h_treeN_rn2_542.
+  exists h_treeN_ln1_2 h_treeN_rn2_3,
+  (0) <= (n1) /\ (0) <= (n2) /\ (n) == (((1) + (n1)) + (n2)) /\ h = x :-> (v) \+ x .+ 1 :-> (l) \+ x .+ 2 :-> (r) \+ h_treeN_ln1_2 \+ h_treeN_rn2_3 /\ treeN l n1 h_treeN_ln1_2 /\ treeN r n2 h_treeN_rn2_3.
 
 
 Inductive tree (x : ptr) (s : seq nat) (h : heap) : Prop :=
@@ -46,5 +47,5 @@ Inductive tree (x : ptr) (s : seq nat) (h : heap) : Prop :=
   (s) == (@nil nat) /\ h = empty
 | tree_2 of ~~ ((x) == (null)) of
   exists (v : nat) (s1 : seq nat) (s2 : seq nat) (l : ptr) (r : ptr),
-  exists h_tree_ls1_539 h_tree_rs2_540,
-  (s) == ((([:: v]) ++ (s1)) ++ (s2)) /\ h = x :-> v \+ x .+ 1 :-> l \+ x .+ 2 :-> r \+ h_tree_ls1_539 \+ h_tree_rs2_540 /\ tree l s1 h_tree_ls1_539 /\ tree r s2 h_tree_rs2_540.
+  exists h_tree_ls1_0 h_tree_rs2_1,
+  (s) == ((([:: v]) ++ (s1)) ++ (s2)) /\ h = x :-> (v) \+ x .+ 1 :-> (l) \+ x .+ 2 :-> (r) \+ h_tree_ls1_0 \+ h_tree_rs2_1 /\ tree l s1 h_tree_ls1_0 /\ tree r s2 h_tree_rs2_1.
