benchmarks/standard/dll/dll_append.v
@@ -8,6 +8,7 @@ From SSL
 Require Import core.
 From Hammer Require Import Hammer.
 (* Configure Hammer *)
+Set Hammer ATPLimit 60.
 Unset Hammer Eprover.
 Unset Hammer Vampire.
 Add Search Blacklist "fcsl.".
@@ -25,10 +26,10 @@ Add Search Blacklist "mathcomp.ssreflect.tuple".
 
 Require Import common.
 
-Lemma pure30 (vx12 : nat) (s1x1 : seq nat) (s2 : seq nat) : ((s1x1) ++ (s2)) = (@nil nat) -> ((([:: vx12]) ++ (s1x1)) ++ (s2)) = ([:: vx12]). intros; hammer. Qed.
-Hint Resolve pure30: ssl_pure.
-Lemma pure31 (s1x1 : seq nat) (s1y12 : seq nat) (s2 : seq nat) (vy122 : nat) (vx12 : nat) : ((s1x1) ++ (s2)) = (([:: vy122]) ++ (s1y12)) -> ((([:: vx12]) ++ (s1x1)) ++ (s2)) = (([:: vx12]) ++ (([:: vy122]) ++ (s1y12))). intros; hammer. Qed.
-Hint Resolve pure31: ssl_pure.
+Lemma pure1 (vx11 : nat) (s1x1 : seq nat) (s2 : seq nat) : ((s1x1) ++ (s2)) = (@nil nat) -> ((([:: vx11]) ++ (s1x1)) ++ (s2)) = ([:: vx11]). intros; hammer. Qed.
+Hint Resolve pure1: ssl_pure.
+Lemma pure2 (s1y11 : seq nat) (s1x1 : seq nat) (s2 : seq nat) (vy111 : nat) (vx11 : nat) : ((s1x1) ++ (s2)) = (([:: vy111]) ++ (s1y11)) -> ((([:: vx11]) ++ (s1x1)) ++ (s2)) = (([:: vx11]) ++ (([:: vy111]) ++ (s1y11))). intros; hammer. Qed.
+Hint Resolve pure2: ssl_pure.
 
 Definition dll_append_type :=
   forall (vprogs : ptr * ptr),
@@ -37,196 +38,196 @@ Definition dll_append_type :=
     fun h =>
       let: (x1, r) := vprogs in
       let: (a, s1, x2, b, s2) := vghosts in
-      exists h_dll_x1as1_536 h_dll_x2bs2_537,
-      h = r :-> x2 \+ h_dll_x1as1_536 \+ h_dll_x2bs2_537 /\ dll x1 a s1 h_dll_x1as1_536 /\ dll x2 b s2 h_dll_x2bs2_537,
+      exists h_dll_x1as1_1 h_dll_x2bs2_2,
+      h = r :-> (x2) \+ h_dll_x1as1_1 \+ h_dll_x2bs2_2 /\ dll x1 a s1 h_dll_x1as1_1 /\ dll x2 b s2 h_dll_x2bs2_2,
     [vfun (_: unit) h =>
       let: (x1, r) := vprogs in
       let: (a, s1, x2, b, s2) := vghosts in
       exists s y c,
-      exists h_dll_ycs_538,
-      (s) == ((s1) ++ (s2)) /\ h = r :-> y \+ h_dll_ycs_538 /\ dll y c s h_dll_ycs_538
+      exists h_dll_ycs_3,
+      (s) == ((s1) ++ (s2)) /\ h = r :-> (y) \+ h_dll_ycs_3 /\ dll y c s h_dll_ycs_3
     ]).
 
 Program Definition dll_append : dll_append_type :=
   Fix (fun (dll_append : dll_append_type) vprogs =>
     let: (x1, r) := vprogs in
     Do (
-      x22 <-- @read ptr r;
+      x21 <-- @read ptr r;
       if (x1) == (null)
       then
         ret tt
       else
-        vx12 <-- @read nat x1;
-        wx12 <-- @read ptr (x1 .+ 1);
-        a2 <-- @read ptr (x1 .+ 2);
-        dll_append (wx12, r);;
-        y12 <-- @read ptr r;
-        if (y12) == (null)
+        vx11 <-- @read nat x1;
+        wx11 <-- @read ptr (x1 .+ 1);
+        a1 <-- @read ptr (x1 .+ 2);
+        dll_append (wx11, r);;
+        y11 <-- @read ptr r;
+        if (y11) == (null)
         then
-          (x1 .+ 1) ::= null;;
           r ::= x1;;
+          (x1 .+ 1) ::= null;;
           ret tt
         else
-          vy122 <-- @read nat y12;
-          wy122 <-- @read ptr (y12 .+ 1);
-          c12 <-- @read ptr (y12 .+ 2);
-          (y12 .+ 2) ::= x1;;
-          (x1 .+ 1) ::= y12;;
+          vy111 <-- @read nat y11;
+          wy111 <-- @read ptr (y11 .+ 1);
+          c11 <-- @read ptr (y11 .+ 2);
+          (y11 .+ 2) ::= x1;;
           r ::= x1;;
+          (x1 .+ 1) ::= y11;;
           ret tt
     )).
 Obligation Tactic := intro; move=>[x1 r]; ssl_program_simpl.
 Next Obligation.
 ssl_ghostelim_pre.
 move=>[[[[a s1] x2] b] s2].
-ex_elim h_dll_x1as1_536 h_dll_x2bs2_537.
+ex_elim h_dll_x1as1_1 h_dll_x2bs2_2.
 move=>[sigma_self].
 subst h_self.
-move=>[H_dll_x1as1_536 H_dll_x2bs2_537].
+move=>[H_dll_x1as1_1 H_dll_x2bs2_2].
 ssl_ghostelim_post.
-try rename h_dll_ycs_538 into h_dll_ycs1s2_538.
-try rename H_dll_ycs_538 into H_dll_ycs1s2_538.
+try rename h_dll_ycs_3 into h_dll_ycs1s2_3.
+try rename H_dll_ycs_3 into H_dll_ycs1s2_3.
 ssl_read r.
-try rename x2 into x22.
-try rename h_dll_x2bs2_537 into h_dll_x22bs2_537.
-try rename H_dll_x2bs2_537 into H_dll_x22bs2_537.
-ssl_open ((x1) == (null)) H_dll_x1as1_536.
-move=>[phi_dll_x1as1_5360].
-move=>[sigma_dll_x1as1_536].
-subst h_dll_x1as1_536.
-try rename h_dll_ycs1s2_538 into h_dll_ycs2_538.
-try rename H_dll_ycs1s2_538 into H_dll_ycs2_538.
-try rename h_dll_x1as1_536 into h_dll_x1a_536.
-try rename H_dll_x1as1_536 into H_dll_x1a_536.
-try rename h_dll_ycs2_538 into h_dll_x22bs2_537.
-try rename H_dll_ycs2_538 into H_dll_x22bs2_537.
+try rename x2 into x21.
+try rename h_dll_x2bs2_2 into h_dll_x21bs2_2.
+try rename H_dll_x2bs2_2 into H_dll_x21bs2_2.
+ssl_open ((x1) == (null)) H_dll_x1as1_1.
+move=>[phi_dll_x1as1_10].
+move=>[sigma_dll_x1as1_1].
+subst h_dll_x1as1_1.
+try rename h_dll_x1as1_1 into h_dll_x1a_1.
+try rename H_dll_x1as1_1 into H_dll_x1a_1.
+try rename h_dll_ycs1s2_3 into h_dll_ycs2_3.
+try rename H_dll_ycs1s2_3 into H_dll_ycs2_3.
+try rename h_dll_ycs2_3 into h_dll_x21bs2_2.
+try rename H_dll_ycs2_3 into H_dll_x21bs2_2.
 ssl_emp;
-exists (s2), (x22), (b);
-exists (h_dll_x22bs2_537);
+exists (s2), (x21), (b);
+exists (h_dll_x21bs2_2);
 sslauto.
 ssl_frame_unfold.
 ex_elim vx1 s1x1 wx1.
-ex_elim h_dll_wx1x1s1x1_535x1.
-move=>[phi_dll_x1as1_5360].
-move=>[sigma_dll_x1as1_536].
-subst h_dll_x1as1_536.
-move=>H_dll_wx1x1s1x1_535x1.
-try rename h_dll_ycs1s2_538 into h_dll_ycvx1s1x1s2_538.
-try rename H_dll_ycs1s2_538 into H_dll_ycvx1s1x1s2_538.
-try rename h_dll_x1as1_536 into h_dll_x1avx1s1x1_536.
-try rename H_dll_x1as1_536 into H_dll_x1avx1s1x1_536.
+ex_elim h_dll_wx1x1s1x1_0x1.
+move=>[phi_dll_x1as1_10].
+move=>[sigma_dll_x1as1_1].
+subst h_dll_x1as1_1.
+move=>H_dll_wx1x1s1x1_0x1.
+try rename h_dll_x1as1_1 into h_dll_x1avx1s1x1_1.
+try rename H_dll_x1as1_1 into H_dll_x1avx1s1x1_1.
+try rename h_dll_ycs1s2_3 into h_dll_ycvx1s1x1s2_3.
+try rename H_dll_ycs1s2_3 into H_dll_ycvx1s1x1s2_3.
 ssl_read x1.
-try rename vx1 into vx12.
-try rename h_dll_x1avx1s1x1_536 into h_dll_x1avx12s1x1_536.
-try rename H_dll_x1avx1s1x1_536 into H_dll_x1avx12s1x1_536.
-try rename h_dll_ycvx1s1x1s2_538 into h_dll_ycvx12s1x1s2_538.
-try rename H_dll_ycvx1s1x1s2_538 into H_dll_ycvx12s1x1s2_538.
+try rename vx1 into vx11.
+try rename h_dll_ycvx1s1x1s2_3 into h_dll_ycvx11s1x1s2_3.
+try rename H_dll_ycvx1s1x1s2_3 into H_dll_ycvx11s1x1s2_3.
+try rename h_dll_x1avx1s1x1_1 into h_dll_x1avx11s1x1_1.
+try rename H_dll_x1avx1s1x1_1 into H_dll_x1avx11s1x1_1.
 ssl_read (x1 .+ 1).
-try rename wx1 into wx12.
-try rename h_dll_wx1x1s1x1_535x1 into h_dll_wx12x1s1x1_535x1.
-try rename H_dll_wx1x1s1x1_535x1 into H_dll_wx12x1s1x1_535x1.
+try rename wx1 into wx11.
+try rename h_dll_wx1x1s1x1_0x1 into h_dll_wx11x1s1x1_0x1.
+try rename H_dll_wx1x1s1x1_0x1 into H_dll_wx11x1s1x1_0x1.
 ssl_read (x1 .+ 2).
-try rename a into a2.
-try rename h_dll_x1avx12s1x1_536 into h_dll_x1a2vx12s1x1_536.
-try rename H_dll_x1avx12s1x1_536 into H_dll_x1a2vx12s1x1_536.
-try rename h_dll_x11a1s11_5361 into h_dll_wx12x1s1x1_535x1.
-try rename H_dll_x11a1s11_5361 into H_dll_wx12x1s1x1_535x1.
-try rename h_dll_x21b1s21_5371 into h_dll_x22bs2_537.
-try rename H_dll_x21b1s21_5371 into H_dll_x22bs2_537.
-ssl_call_pre (r :-> x22 \+ h_dll_wx12x1s1x1_535x1 \+ h_dll_x22bs2_537).
-ssl_call (x1, s1x1, x22, b, s2).
-exists (h_dll_wx12x1s1x1_535x1), (h_dll_x22bs2_537);
+try rename a into a1.
+try rename h_dll_x1avx11s1x1_1 into h_dll_x1a1vx11s1x1_1.
+try rename H_dll_x1avx11s1x1_1 into H_dll_x1a1vx11s1x1_1.
+try rename h_dll_x11a2s11_11 into h_dll_wx11x1s1x1_0x1.
+try rename H_dll_x11a2s11_11 into H_dll_wx11x1s1x1_0x1.
+try rename h_dll_x22b1s21_21 into h_dll_x21bs2_2.
+try rename H_dll_x22b1s21_21 into H_dll_x21bs2_2.
+ssl_call_pre (r :-> (x21) \+ h_dll_wx11x1s1x1_0x1 \+ h_dll_x21bs2_2).
+ssl_call (x1, s1x1, x21, b, s2).
+exists (h_dll_wx11x1s1x1_0x1), (h_dll_x21bs2_2);
 sslauto.
 ssl_frame_unfold.
 ssl_frame_unfold.
 move=>h_call0.
 ex_elim s3 y1 c1.
-ex_elim h_dll_y1c1s3_5381.
+ex_elim h_dll_y1c1s3_31.
 move=>[phi_call00].
 move=>[sigma_call0].
 subst h_call0.
-move=>H_dll_y1c1s3_5381.
+move=>H_dll_y1c1s3_31.
 store_valid.
-try rename h_dll_y1c1s3_5381 into h_dll_y1c1s1x1s2_5381.
-try rename H_dll_y1c1s3_5381 into H_dll_y1c1s1x1s2_5381.
+try rename h_dll_y1c1s3_31 into h_dll_y1c1s1x1s2_31.
+try rename H_dll_y1c1s3_31 into H_dll_y1c1s1x1s2_31.
 ssl_read r.
-try rename y1 into y12.
-try rename h_dll_y1c1s1x1s2_5381 into h_dll_y12c1s1x1s2_5381.
-try rename H_dll_y1c1s1x1s2_5381 into H_dll_y12c1s1x1s2_5381.
-ssl_open ((y12) == (null)) H_dll_y12c1s1x1s2_5381.
-move=>[phi_dll_y12c1s1x1s2_53810].
-move=>[sigma_dll_y12c1s1x1s2_5381].
-subst h_dll_y12c1s1x1s2_5381.
-try rename h_dll_wyys12y_535y into h_dll_wyy_535y.
-try rename H_dll_wyys12y_535y into H_dll_wyy_535y.
-try rename h_dll_wyy_535y into h_dll_y_535y.
-try rename H_dll_wyy_535y into H_dll_y_535y.
-try rename h_dll_ycvx12s1x1s2_538 into h_dll_x1cvx12s1x1s2_538.
-try rename H_dll_ycvx12s1x1s2_538 into H_dll_x1cvx12s1x1s2_538.
-try rename h_dll_y_535y into h_dll_x1_535y.
-try rename H_dll_y_535y into H_dll_x1_535y.
-ssl_write (x1 .+ 1).
-ssl_write_post (x1 .+ 1).
+try rename y1 into y11.
+try rename h_dll_y1c1s1x1s2_31 into h_dll_y11c1s1x1s2_31.
+try rename H_dll_y1c1s1x1s2_31 into H_dll_y11c1s1x1s2_31.
+ssl_open ((y11) == (null)) H_dll_y11c1s1x1s2_31.
+move=>[phi_dll_y11c1s1x1s2_310].
+move=>[sigma_dll_y11c1s1x1s2_31].
+subst h_dll_y11c1s1x1s2_31.
+try rename h_dll_wyys12y_0y into h_dll_wyy_0y.
+try rename H_dll_wyys12y_0y into H_dll_wyy_0y.
+try rename h_dll_wyy_0y into h_dll_y_0y.
+try rename H_dll_wyy_0y into H_dll_y_0y.
+try rename h_dll_ycvx11s1x1s2_3 into h_dll_x1cvx11s1x1s2_3.
+try rename H_dll_ycvx11s1x1s2_3 into H_dll_x1cvx11s1x1s2_3.
+try rename h_dll_y_0y into h_dll_x1_0y.
+try rename H_dll_y_0y into H_dll_x1_0y.
 ssl_write r.
 ssl_write_post r.
-try rename h_dll_x1cvx12s1x1s2_538 into h_dll_x1a2vx12s1x1s2_538.
-try rename H_dll_x1cvx12s1x1s2_538 into H_dll_x1a2vx12s1x1s2_538.
+ssl_write (x1 .+ 1).
+ssl_write_post (x1 .+ 1).
+try rename h_dll_x1cvx11s1x1s2_3 into h_dll_x1a1vx11s1x1s2_3.
+try rename H_dll_x1cvx11s1x1s2_3 into H_dll_x1a1vx11s1x1s2_3.
 ssl_emp;
-exists ((([:: vx12]) ++ (s1x1)) ++ (s2)), (x1), (a2);
-exists (x1 :-> vx12 \+ x1 .+ 1 :-> null \+ x1 .+ 2 :-> a2);
+exists ((([:: vx11]) ++ (s1x1)) ++ (s2)), (x1), (a1);
+exists (x1 :-> (vx11) \+ x1 .+ 1 :-> (null) \+ x1 .+ 2 :-> (a1));
 sslauto.
 ssl_close 2;
-exists (vx12), (@nil nat), (null), (empty);
+exists (vx11), (@nil nat), (null), (empty);
 sslauto.
 ssl_close 1;
 sslauto.
-ex_elim vy12 s1y12 wy12.
-ex_elim h_dll_wy12y12s1y12_535y12.
-move=>[phi_dll_y12c1s1x1s2_53810].
-move=>[sigma_dll_y12c1s1x1s2_5381].
-subst h_dll_y12c1s1x1s2_5381.
-move=>H_dll_wy12y12s1y12_535y12.
-ssl_read y12.
-try rename vy12 into vy122.
-ssl_read (y12 .+ 1).
-try rename wy12 into wy122.
-try rename h_dll_wy12y12s1y12_535y12 into h_dll_wy122y12s1y12_535y12.
-try rename H_dll_wy12y12s1y12_535y12 into H_dll_wy122y12s1y12_535y12.
-ssl_read (y12 .+ 2).
-try rename c1 into c12.
-try rename h_dll_y12c1s1x1s2_5381 into h_dll_y12c12s1x1s2_5381.
-try rename H_dll_y12c1s1x1s2_5381 into H_dll_y12c12s1x1s2_5381.
-try rename h_dll_wyys12y_535y into h_dll_wyyvwys12wy_535y.
-try rename H_dll_wyys12y_535y into H_dll_wyyvwys12wy_535y.
-try rename h_dll_wwywys12wy_535wy into h_dll_wy122y12s1y12_535y12.
-try rename H_dll_wwywys12wy_535wy into H_dll_wy122y12s1y12_535y12.
-try rename h_dll_wyyvwys12wy_535y into h_dll_wyyvwys1y12_535y.
-try rename H_dll_wyyvwys12wy_535y into H_dll_wyyvwys1y12_535y.
-try rename h_dll_wyyvwys1y12_535y into h_dll_y12yvwys1y12_535y.
-try rename H_dll_wyyvwys1y12_535y into H_dll_y12yvwys1y12_535y.
-try rename h_dll_ycvx12s1x1s2_538 into h_dll_x1cvx12s1x1s2_538.
-try rename H_dll_ycvx12s1x1s2_538 into H_dll_x1cvx12s1x1s2_538.
-try rename h_dll_y12yvwys1y12_535y into h_dll_y12x1vwys1y12_535y.
-try rename H_dll_y12yvwys1y12_535y into H_dll_y12x1vwys1y12_535y.
-ssl_write (y12 .+ 2).
-ssl_write_post (y12 .+ 2).
-ssl_write (x1 .+ 1).
-ssl_write_post (x1 .+ 1).
+ex_elim vy11 s1y11 wy11.
+ex_elim h_dll_wy11y11s1y11_0y11.
+move=>[phi_dll_y11c1s1x1s2_310].
+move=>[sigma_dll_y11c1s1x1s2_31].
+subst h_dll_y11c1s1x1s2_31.
+move=>H_dll_wy11y11s1y11_0y11.
+ssl_read y11.
+try rename vy11 into vy111.
+ssl_read (y11 .+ 1).
+try rename wy11 into wy111.
+try rename h_dll_wy11y11s1y11_0y11 into h_dll_wy111y11s1y11_0y11.
+try rename H_dll_wy11y11s1y11_0y11 into H_dll_wy111y11s1y11_0y11.
+ssl_read (y11 .+ 2).
+try rename c1 into c11.
+try rename h_dll_y11c1s1x1s2_31 into h_dll_y11c11s1x1s2_31.
+try rename H_dll_y11c1s1x1s2_31 into H_dll_y11c11s1x1s2_31.
+try rename h_dll_wyys12y_0y into h_dll_wyyvwys12wy_0y.
+try rename H_dll_wyys12y_0y into H_dll_wyyvwys12wy_0y.
+try rename h_dll_wwywys12wy_0wy into h_dll_wy111y11s1y11_0y11.
+try rename H_dll_wwywys12wy_0wy into H_dll_wy111y11s1y11_0y11.
+try rename h_dll_wyyvwys12wy_0y into h_dll_wyyvwys1y11_0y.
+try rename H_dll_wyyvwys12wy_0y into H_dll_wyyvwys1y11_0y.
+try rename h_dll_wyyvwys1y11_0y into h_dll_y11yvwys1y11_0y.
+try rename H_dll_wyyvwys1y11_0y into H_dll_y11yvwys1y11_0y.
+try rename h_dll_y11yvwys1y11_0y into h_dll_y11x1vwys1y11_0y.
+try rename H_dll_y11yvwys1y11_0y into H_dll_y11x1vwys1y11_0y.
+try rename h_dll_ycvx11s1x1s2_3 into h_dll_x1cvx11s1x1s2_3.
+try rename H_dll_ycvx11s1x1s2_3 into H_dll_x1cvx11s1x1s2_3.
+ssl_write (y11 .+ 2).
+ssl_write_post (y11 .+ 2).
 ssl_write r.
 ssl_write_post r.
-try rename h_dll_x1cvx12s1x1s2_538 into h_dll_x1a2vx12s1x1s2_538.
-try rename H_dll_x1cvx12s1x1s2_538 into H_dll_x1a2vx12s1x1s2_538.
-try rename h_dll_y12x1vwys1y12_535y into h_dll_y12x1vy122s1y12_535y.
-try rename H_dll_y12x1vwys1y12_535y into H_dll_y12x1vy122s1y12_535y.
+ssl_write (x1 .+ 1).
+ssl_write_post (x1 .+ 1).
+try rename h_dll_x1cvx11s1x1s2_3 into h_dll_x1a1vx11s1x1s2_3.
+try rename H_dll_x1cvx11s1x1s2_3 into H_dll_x1a1vx11s1x1s2_3.
+try rename h_dll_y11x1vwys1y11_0y into h_dll_y11x1vy111s1y11_0y.
+try rename H_dll_y11x1vwys1y11_0y into H_dll_y11x1vy111s1y11_0y.
 ssl_emp;
-exists ((([:: vx12]) ++ (s1x1)) ++ (s2)), (x1), (a2);
-exists (x1 :-> vx12 \+ x1 .+ 1 :-> y12 \+ x1 .+ 2 :-> a2 \+ y12 :-> vy122 \+ y12 .+ 1 :-> wy122 \+ y12 .+ 2 :-> x1 \+ h_dll_wy122y12s1y12_535y12);
+exists ((([:: vx11]) ++ (s1x1)) ++ (s2)), (x1), (a1);
+exists (x1 :-> (vx11) \+ x1 .+ 1 :-> (y11) \+ x1 .+ 2 :-> (a1) \+ y11 :-> (vy111) \+ y11 .+ 1 :-> (wy111) \+ y11 .+ 2 :-> (x1) \+ h_dll_wy111y11s1y11_0y11);
 sslauto.
 ssl_close 2;
-exists (vx12), (([:: vy122]) ++ (s1y12)), (y12), (y12 :-> vy122 \+ y12 .+ 1 :-> wy122 \+ y12 .+ 2 :-> x1 \+ h_dll_wy122y12s1y12_535y12);
+exists (vx11), (([:: vy111]) ++ (s1y11)), (y11), (y11 :-> (vy111) \+ y11 .+ 1 :-> (wy111) \+ y11 .+ 2 :-> (x1) \+ h_dll_wy111y11s1y11_0y11);
 sslauto.
 ssl_close 2;
-exists (vy122), (s1y12), (wy122), (h_dll_wy122y12s1y12_535y12);
+exists (vy111), (s1y11), (wy111), (h_dll_wy111y11s1y11_0y11);
 sslauto.
 ssl_frame_unfold.
 Qed.
