benchmarks/standard/dll/dll_singleton.v
@@ -8,6 +8,7 @@ From SSL
 Require Import core.
 From Hammer Require Import Hammer.
 (* Configure Hammer *)
+Set Hammer ATPLimit 60.
 Unset Hammer Eprover.
 Unset Hammer Vampire.
 Add Search Blacklist "fcsl.".
@@ -25,8 +26,8 @@ Add Search Blacklist "mathcomp.ssreflect.tuple".
 
 Require Import common.
 
-Lemma pure29 (x : nat) : ([:: x]) = ([:: x]). intros; hammer. Qed.
-Hint Resolve pure29: ssl_pure.
+Lemma pure1 (x : nat) : ([:: x]) = ([:: x]). intros; hammer. Qed.
+Hint Resolve pure1: ssl_pure.
 
 Definition dll_singleton_type :=
   forall (vprogs : nat * ptr),
@@ -35,25 +36,25 @@ Definition dll_singleton_type :=
     fun h =>
       let: (x, r) := vprogs in
       let: (a) := vghosts in
-      h = r :-> a,
+      h = r :-> (a),
     [vfun (_: unit) h =>
       let: (x, r) := vprogs in
       let: (a) := vghosts in
       exists elems y,
-      exists h_dll_yelems_534,
-      (elems) == ([:: x]) /\ h = r :-> y \+ h_dll_yelems_534 /\ dll y null elems h_dll_yelems_534
+      exists h_dll_yelems_1,
+      (elems) == ([:: x]) /\ h = r :-> (y) \+ h_dll_yelems_1 /\ dll y null elems h_dll_yelems_1
     ]).
 
 Program Definition dll_singleton : dll_singleton_type :=
   Fix (fun (dll_singleton : dll_singleton_type) vprogs =>
     let: (x, r) := vprogs in
     Do (
-      a2 <-- @read ptr r;
-      y2 <-- allocb null 3;
-      r ::= y2;;
-      (y2 .+ 1) ::= null;;
-      (y2 .+ 2) ::= null;;
-      y2 ::= x;;
+      a1 <-- @read ptr r;
+      y1 <-- allocb null 3;
+      r ::= y1;;
+      (y1 .+ 1) ::= null;;
+      (y1 .+ 2) ::= null;;
+      y1 ::= x;;
       ret tt
     )).
 Obligation Tactic := intro; move=>[x r]; ssl_program_simpl.
@@ -63,31 +64,31 @@ move=>a.
 move=>[sigma_self].
 subst h_self.
 ssl_ghostelim_post.
-try rename h_dll_yelems_534 into h_dll_yx_534.
-try rename H_dll_yelems_534 into H_dll_yx_534.
+try rename h_dll_yelems_1 into h_dll_yx_1.
+try rename H_dll_yelems_1 into H_dll_yx_1.
 ssl_read r.
-try rename a into a2.
-try rename h_dll_wyys1y_533y into h_dll_wyy_533y.
-try rename H_dll_wyys1y_533y into H_dll_wyy_533y.
-try rename h_dll_wyy_533y into h_dll_y_533y.
-try rename H_dll_wyy_533y into H_dll_y_533y.
-ssl_alloc y2.
-try rename y into y2.
-try rename h_dll_yx_534 into h_dll_y2x_534.
-try rename H_dll_yx_534 into H_dll_y2x_534.
-try rename h_dll_y_533y into h_dll_y2_533y.
-try rename H_dll_y_533y into H_dll_y2_533y.
+try rename a into a1.
+try rename h_dll_wyys1y_0y into h_dll_wyy_0y.
+try rename H_dll_wyys1y_0y into H_dll_wyy_0y.
+try rename h_dll_wyy_0y into h_dll_y_0y.
+try rename H_dll_wyy_0y into H_dll_y_0y.
+ssl_alloc y1.
+try rename y into y1.
+try rename h_dll_yx_1 into h_dll_y1x_1.
+try rename H_dll_yx_1 into H_dll_y1x_1.
+try rename h_dll_y_0y into h_dll_y1_0y.
+try rename H_dll_y_0y into H_dll_y1_0y.
 ssl_write r.
 ssl_write_post r.
-ssl_write (y2 .+ 1).
-ssl_write_post (y2 .+ 1).
-ssl_write (y2 .+ 2).
-ssl_write_post (y2 .+ 2).
-ssl_write y2.
-ssl_write_post y2.
+ssl_write (y1 .+ 1).
+ssl_write_post (y1 .+ 1).
+ssl_write (y1 .+ 2).
+ssl_write_post (y1 .+ 2).
+ssl_write y1.
+ssl_write_post y1.
 ssl_emp;
-exists ([:: x]), (y2);
-exists (y2 :-> x \+ y2 .+ 1 :-> null \+ y2 .+ 2 :-> null);
+exists ([:: x]), (y1);
+exists (y1 :-> (x) \+ y1 .+ 1 :-> (null) \+ y1 .+ 2 :-> (null));
 sslauto.
 ssl_close 2;
 exists (x), (@nil nat), (null), (empty);
