benchmarks/standard/ints/swap4.v
@@ -8,6 +8,7 @@ From SSL
 Require Import core.
 From Hammer Require Import Hammer.
 (* Configure Hammer *)
+Set Hammer ATPLimit 60.
 Unset Hammer Eprover.
 Unset Hammer Vampire.
 Add Search Blacklist "fcsl.".
@@ -32,25 +33,25 @@ Definition swap4_type :=
     fun h =>
       let: (x, z, y, t) := vprogs in
       let: (a, c, b, q) := vghosts in
-      h = x :-> a \+ y :-> c \+ z :-> b \+ t :-> q,
+      h = x :-> (a) \+ y :-> (c) \+ z :-> (b) \+ t :-> (q),
     [vfun (_: unit) h =>
       let: (x, z, y, t) := vprogs in
       let: (a, c, b, q) := vghosts in
-      h = x :-> q \+ z :-> c \+ t :-> a \+ y :-> b
+      h = x :-> (q) \+ z :-> (c) \+ t :-> (a) \+ y :-> (b)
     ]).
 
 Program Definition swap4 : swap4_type :=
   Fix (fun (swap4 : swap4_type) vprogs =>
     let: (x, z, y, t) := vprogs in
     Do (
-      a2 <-- @read ptr x;
-      c2 <-- @read ptr y;
-      b2 <-- @read ptr z;
-      q2 <-- @read ptr t;
-      x ::= q2;;
-      y ::= b2;;
-      z ::= c2;;
-      t ::= a2;;
+      a1 <-- @read ptr x;
+      c1 <-- @read ptr y;
+      b1 <-- @read ptr z;
+      q1 <-- @read ptr t;
+      t ::= a1;;
+      z ::= c1;;
+      y ::= b1;;
+      x ::= q1;;
       ret tt
     )).
 Obligation Tactic := intro; move=>[[[x z] y] t]; ssl_program_simpl.
@@ -61,21 +62,21 @@ move=>[sigma_self].
 subst h_self.
 ssl_ghostelim_post.
 ssl_read x.
-try rename a into a2.
+try rename a into a1.
 ssl_read y.
-try rename c into c2.
+try rename c into c1.
 ssl_read z.
-try rename b into b2.
+try rename b into b1.
 ssl_read t.
-try rename q into q2.
-ssl_write x.
-ssl_write_post x.
-ssl_write y.
-ssl_write_post y.
-ssl_write z.
-ssl_write_post z.
+try rename q into q1.
 ssl_write t.
 ssl_write_post t.
+ssl_write z.
+ssl_write_post z.
+ssl_write y.
+ssl_write_post y.
+ssl_write x.
+ssl_write_post x.
 ssl_emp;
 sslauto.
 Qed.
