benchmarks/standard/sll-bounds/common.v
@@ -8,6 +8,7 @@ From SSL
 Require Import core.
 From Hammer Require Import Hammer.
 (* Configure Hammer *)
+Set Hammer ATPLimit 60.
 Unset Hammer Eprover.
 Unset Hammer Vampire.
 Add Search Blacklist "fcsl.".
@@ -28,5 +29,5 @@ Inductive sll (x : ptr) (len : nat) (lo : nat) (hi : nat) (h : heap) : Prop :=
   (hi) == (0) /\ (len) == (0) /\ (lo) == (7) /\ h = empty
 | sll_2 of ~~ ((x) == (null)) of
   exists (len1 : nat) (v : nat) (hi1 : nat) (lo1 : nat) (nxt : ptr),
-  exists h_sll_nxtlen1lo1hi1_513,
-  (0) <= (len1) /\ (0) <= (v) /\ (hi) == ((if (hi1) <= (v) then v else hi1)) /\ (len) == ((1) + (len1)) /\ (lo) == ((if (v) <= (lo1) then v else lo1)) /\ (v) <= (7) /\ h = x :-> v \+ x .+ 1 :-> nxt \+ h_sll_nxtlen1lo1hi1_513 /\ sll nxt len1 lo1 hi1 h_sll_nxtlen1lo1hi1_513.
+  exists h_sll_nxtlen1lo1hi1_0,
+  (0) <= (len1) /\ (0) <= (v) /\ (hi) == ((if (hi1) <= (v) then v else hi1)) /\ (len) == ((1) + (len1)) /\ (lo) == ((if (v) <= (lo1) then v else lo1)) /\ (v) <= (7) /\ h = x :-> (v) \+ x .+ 1 :-> (nxt) \+ h_sll_nxtlen1lo1hi1_0 /\ sll nxt len1 lo1 hi1 h_sll_nxtlen1lo1hi1_0.
