benchmarks/standard/sll-bounds/sll_min.v
@@ -8,6 +8,7 @@ From SSL
 Require Import core.
 From Hammer Require Import Hammer.
 (* Configure Hammer *)
+Set Hammer ATPLimit 60.
 Unset Hammer Eprover.
 Unset Hammer Vampire.
 Add Search Blacklist "fcsl.".
@@ -25,16 +26,16 @@ Add Search Blacklist "mathcomp.ssreflect.tuple".
 
 Require Import common.
 
-Lemma pure7 : (0) = (0). intros; hammer. Qed.
-Hint Resolve pure7: ssl_pure.
-Lemma pure8 : (7) = (7). intros; hammer. Qed.
-Hint Resolve pure8: ssl_pure.
-Lemma pure9 (len1x : nat) : (0) <= (len1x) -> ((1) + (len1x)) = ((1) + (len1x)). intros; hammer. Qed.
-Hint Resolve pure9: ssl_pure.
-Lemma pure10 (hi1x : nat) (vx2 : nat) : (0) <= (vx2) -> (vx2) <= (7) -> ((if (hi1x) <= (vx2) then vx2 else hi1x)) = ((if (hi1x) <= (vx2) then vx2 else hi1x)). intros; hammer. Qed.
-Hint Resolve pure10: ssl_pure.
-Lemma pure11 (vx2 : nat) (lo1x2 : nat) : (0) <= (vx2) -> (vx2) <= (7) -> ((if (vx2) <= (lo1x2) then vx2 else lo1x2)) = ((if (vx2) <= (lo1x2) then vx2 else lo1x2)). intros; hammer. Qed.
-Hint Resolve pure11: ssl_pure.
+Lemma pure1 : (0) = (0). intros; hammer. Qed.
+Hint Resolve pure1: ssl_pure.
+Lemma pure2 : (7) = (7). intros; hammer. Qed.
+Hint Resolve pure2: ssl_pure.
+Lemma pure3 (len1x : nat) : (0) <= (len1x) -> ((1) + (len1x)) = ((1) + (len1x)). intros; hammer. Qed.
+Hint Resolve pure3: ssl_pure.
+Lemma pure4 (hi1x : nat) (vx1 : nat) : (vx1) <= (7) -> (0) <= (vx1) -> ((if (hi1x) <= (vx1) then vx1 else hi1x)) = ((if (hi1x) <= (vx1) then vx1 else hi1x)). intros; hammer. Qed.
+Hint Resolve pure4: ssl_pure.
+Lemma pure5 (vx1 : nat) (lo1x1 : nat) : (vx1) <= (7) -> (0) <= (vx1) -> ((if (vx1) <= (lo1x1) then vx1 else lo1x1)) = ((if (vx1) <= (lo1x1) then vx1 else lo1x1)). intros; hammer. Qed.
+Hint Resolve pure5: ssl_pure.
 
 Definition sll_min_type :=
   forall (vprogs : ptr * ptr),
@@ -43,59 +44,59 @@ Definition sll_min_type :=
     fun h =>
       let: (x, r) := vprogs in
       let: (n, lo, hi, a) := vghosts in
-      exists h_sll_xnlohi_514,
-      h = r :-> a \+ h_sll_xnlohi_514 /\ sll x n lo hi h_sll_xnlohi_514,
+      exists h_sll_xnlohi_1,
+      h = r :-> (a) \+ h_sll_xnlohi_1 /\ sll x n lo hi h_sll_xnlohi_1,
     [vfun (_: unit) h =>
       let: (x, r) := vprogs in
       let: (n, lo, hi, a) := vghosts in
-      exists h_sll_xnlohi_515,
-      h = r :-> lo \+ h_sll_xnlohi_515 /\ sll x n lo hi h_sll_xnlohi_515
+      exists h_sll_xnlohi_2,
+      h = r :-> (lo) \+ h_sll_xnlohi_2 /\ sll x n lo hi h_sll_xnlohi_2
     ]).
 
 Program Definition sll_min : sll_min_type :=
   Fix (fun (sll_min : sll_min_type) vprogs =>
     let: (x, r) := vprogs in
     Do (
-      a2 <-- @read ptr r;
+      a1 <-- @read ptr r;
       if (x) == (null)
       then
         r ::= 7;;
         ret tt
       else
-        vx2 <-- @read nat x;
-        nxtx2 <-- @read ptr (x .+ 1);
-        sll_min (nxtx2, r);;
-        lo1x2 <-- @read nat r;
-        r ::= (if (vx2) <= (lo1x2) then vx2 else lo1x2);;
+        vx1 <-- @read nat x;
+        nxtx1 <-- @read ptr (x .+ 1);
+        sll_min (nxtx1, r);;
+        lo1x1 <-- @read nat r;
+        r ::= (if (vx1) <= (lo1x1) then vx1 else lo1x1);;
         ret tt
     )).
 Obligation Tactic := intro; move=>[x r]; ssl_program_simpl.
 Next Obligation.
 ssl_ghostelim_pre.
 move=>[[[n lo] hi] a].
-ex_elim h_sll_xnlohi_514.
+ex_elim h_sll_xnlohi_1.
 move=>[sigma_self].
 subst h_self.
-move=>H_sll_xnlohi_514.
+move=>H_sll_xnlohi_1.
 ssl_ghostelim_post.
 ssl_read r.
-try rename a into a2.
-ssl_open ((x) == (null)) H_sll_xnlohi_514.
-move=>[phi_sll_xnlohi_5140] [phi_sll_xnlohi_5141] [phi_sll_xnlohi_5142].
-move=>[sigma_sll_xnlohi_514].
-subst h_sll_xnlohi_514.
-try rename h_sll_xnlohi_514 into h_sll_xnlo_514.
-try rename H_sll_xnlohi_514 into H_sll_xnlo_514.
-try rename h_sll_xnlohi_515 into h_sll_xnlo_515.
-try rename H_sll_xnlohi_515 into H_sll_xnlo_515.
-try rename h_sll_xnlo_514 into h_sll_xn_514.
-try rename H_sll_xnlo_514 into H_sll_xn_514.
-try rename h_sll_xnlo_515 into h_sll_xn_515.
-try rename H_sll_xnlo_515 into H_sll_xn_515.
-try rename h_sll_xn_515 into h_sll_x_515.
-try rename H_sll_xn_515 into H_sll_x_515.
-try rename h_sll_xn_514 into h_sll_x_514.
-try rename H_sll_xn_514 into H_sll_x_514.
+try rename a into a1.
+ssl_open ((x) == (null)) H_sll_xnlohi_1.
+move=>[phi_sll_xnlohi_10] [phi_sll_xnlohi_11] [phi_sll_xnlohi_12].
+move=>[sigma_sll_xnlohi_1].
+subst h_sll_xnlohi_1.
+try rename h_sll_xnlohi_1 into h_sll_xnlo_1.
+try rename H_sll_xnlohi_1 into H_sll_xnlo_1.
+try rename h_sll_xnlohi_2 into h_sll_xnlo_2.
+try rename H_sll_xnlohi_2 into H_sll_xnlo_2.
+try rename h_sll_xnlo_1 into h_sll_xn_1.
+try rename H_sll_xnlo_1 into H_sll_xn_1.
+try rename h_sll_xnlo_2 into h_sll_xn_2.
+try rename H_sll_xnlo_2 into H_sll_xn_2.
+try rename h_sll_xn_2 into h_sll_x_2.
+try rename H_sll_xn_2 into H_sll_x_2.
+try rename h_sll_xn_1 into h_sll_x_1.
+try rename H_sll_xn_1 into H_sll_x_1.
 ssl_write r.
 ssl_write_post r.
 ssl_emp;
@@ -104,65 +105,65 @@ sslauto.
 ssl_close 1;
 sslauto.
 ex_elim len1x vx hi1x lo1x nxtx.
-ex_elim h_sll_nxtxlen1xlo1xhi1x_513x.
-move=>[phi_sll_xnlohi_5140] [phi_sll_xnlohi_5141] [phi_sll_xnlohi_5142] [phi_sll_xnlohi_5143] [phi_sll_xnlohi_5144] [phi_sll_xnlohi_5145].
-move=>[sigma_sll_xnlohi_514].
-subst h_sll_xnlohi_514.
-move=>H_sll_nxtxlen1xlo1xhi1x_513x.
-try rename h_sll_xnlohi_514 into h_sll_xnlohi1xvxvxhi1x_514.
-try rename H_sll_xnlohi_514 into H_sll_xnlohi1xvxvxhi1x_514.
-try rename h_sll_xnlohi_515 into h_sll_xnlohi1xvxvxhi1x_515.
-try rename H_sll_xnlohi_515 into H_sll_xnlohi1xvxvxhi1x_515.
-try rename h_sll_xnlohi1xvxvxhi1x_514 into h_sll_xnvxlo1xvxlo1xhi1xvxvxhi1x_514.
-try rename H_sll_xnlohi1xvxvxhi1x_514 into H_sll_xnvxlo1xvxlo1xhi1xvxvxhi1x_514.
-try rename h_sll_xnlohi1xvxvxhi1x_515 into h_sll_xnvxlo1xvxlo1xhi1xvxvxhi1x_515.
-try rename H_sll_xnlohi1xvxvxhi1x_515 into H_sll_xnvxlo1xvxlo1xhi1xvxvxhi1x_515.
-try rename h_sll_xnvxlo1xvxlo1xhi1xvxvxhi1x_515 into h_sll_xlen1xvxlo1xvxlo1xhi1xvxvxhi1x_515.
-try rename H_sll_xnvxlo1xvxlo1xhi1xvxvxhi1x_515 into H_sll_xlen1xvxlo1xvxlo1xhi1xvxvxhi1x_515.
-try rename h_sll_xnvxlo1xvxlo1xhi1xvxvxhi1x_514 into h_sll_xlen1xvxlo1xvxlo1xhi1xvxvxhi1x_514.
-try rename H_sll_xnvxlo1xvxlo1xhi1xvxvxhi1x_514 into H_sll_xlen1xvxlo1xvxlo1xhi1xvxvxhi1x_514.
+ex_elim h_sll_nxtxlen1xlo1xhi1x_0x.
+move=>[phi_sll_xnlohi_10] [phi_sll_xnlohi_11] [phi_sll_xnlohi_12] [phi_sll_xnlohi_13] [phi_sll_xnlohi_14] [phi_sll_xnlohi_15].
+move=>[sigma_sll_xnlohi_1].
+subst h_sll_xnlohi_1.
+move=>H_sll_nxtxlen1xlo1xhi1x_0x.
+try rename h_sll_xnlohi_1 into h_sll_xnlohi1xvxvxhi1x_1.
+try rename H_sll_xnlohi_1 into H_sll_xnlohi1xvxvxhi1x_1.
+try rename h_sll_xnlohi_2 into h_sll_xnlohi1xvxvxhi1x_2.
+try rename H_sll_xnlohi_2 into H_sll_xnlohi1xvxvxhi1x_2.
+try rename h_sll_xnlohi1xvxvxhi1x_2 into h_sll_xnvxlo1xvxlo1xhi1xvxvxhi1x_2.
+try rename H_sll_xnlohi1xvxvxhi1x_2 into H_sll_xnvxlo1xvxlo1xhi1xvxvxhi1x_2.
+try rename h_sll_xnlohi1xvxvxhi1x_1 into h_sll_xnvxlo1xvxlo1xhi1xvxvxhi1x_1.
+try rename H_sll_xnlohi1xvxvxhi1x_1 into H_sll_xnvxlo1xvxlo1xhi1xvxvxhi1x_1.
+try rename h_sll_xnvxlo1xvxlo1xhi1xvxvxhi1x_2 into h_sll_xlen1xvxlo1xvxlo1xhi1xvxvxhi1x_2.
+try rename H_sll_xnvxlo1xvxlo1xhi1xvxvxhi1x_2 into H_sll_xlen1xvxlo1xvxlo1xhi1xvxvxhi1x_2.
+try rename h_sll_xnvxlo1xvxlo1xhi1xvxvxhi1x_1 into h_sll_xlen1xvxlo1xvxlo1xhi1xvxvxhi1x_1.
+try rename H_sll_xnvxlo1xvxlo1xhi1xvxvxhi1x_1 into H_sll_xlen1xvxlo1xvxlo1xhi1xvxvxhi1x_1.
 ssl_read x.
-try rename vx into vx2.
-try rename h_sll_xlen1xvxlo1xvxlo1xhi1xvxvxhi1x_515 into h_sll_xlen1xvx2lo1xvx2lo1xhi1xvx2vx2hi1x_515.
-try rename H_sll_xlen1xvxlo1xvxlo1xhi1xvxvxhi1x_515 into H_sll_xlen1xvx2lo1xvx2lo1xhi1xvx2vx2hi1x_515.
-try rename h_sll_xlen1xvxlo1xvxlo1xhi1xvxvxhi1x_514 into h_sll_xlen1xvx2lo1xvx2lo1xhi1xvx2vx2hi1x_514.
-try rename H_sll_xlen1xvxlo1xvxlo1xhi1xvxvxhi1x_514 into H_sll_xlen1xvx2lo1xvx2lo1xhi1xvx2vx2hi1x_514.
+try rename vx into vx1.
+try rename h_sll_xlen1xvxlo1xvxlo1xhi1xvxvxhi1x_1 into h_sll_xlen1xvx1lo1xvx1lo1xhi1xvx1vx1hi1x_1.
+try rename H_sll_xlen1xvxlo1xvxlo1xhi1xvxvxhi1x_1 into H_sll_xlen1xvx1lo1xvx1lo1xhi1xvx1vx1hi1x_1.
+try rename h_sll_xlen1xvxlo1xvxlo1xhi1xvxvxhi1x_2 into h_sll_xlen1xvx1lo1xvx1lo1xhi1xvx1vx1hi1x_2.
+try rename H_sll_xlen1xvxlo1xvxlo1xhi1xvxvxhi1x_2 into H_sll_xlen1xvx1lo1xvx1lo1xhi1xvx1vx1hi1x_2.
 ssl_read (x .+ 1).
-try rename nxtx into nxtx2.
-try rename h_sll_nxtxlen1xlo1xhi1x_513x into h_sll_nxtx2len1xlo1xhi1x_513x.
-try rename H_sll_nxtxlen1xlo1xhi1x_513x into H_sll_nxtx2len1xlo1xhi1x_513x.
-try rename h_sll_x1n1lo1hi1_5141 into h_sll_nxtx2len1xlo1xhi1x_513x.
-try rename H_sll_x1n1lo1hi1_5141 into H_sll_nxtx2len1xlo1xhi1x_513x.
-ssl_call_pre (r :-> a2 \+ h_sll_nxtx2len1xlo1xhi1x_513x).
-ssl_call (len1x, lo1x, hi1x, a2).
-exists (h_sll_nxtx2len1xlo1xhi1x_513x);
+try rename nxtx into nxtx1.
+try rename h_sll_nxtxlen1xlo1xhi1x_0x into h_sll_nxtx1len1xlo1xhi1x_0x.
+try rename H_sll_nxtxlen1xlo1xhi1x_0x into H_sll_nxtx1len1xlo1xhi1x_0x.
+try rename h_sll_x1n1lo1hi1_11 into h_sll_nxtx1len1xlo1xhi1x_0x.
+try rename H_sll_x1n1lo1hi1_11 into H_sll_nxtx1len1xlo1xhi1x_0x.
+ssl_call_pre (r :-> (a1) \+ h_sll_nxtx1len1xlo1xhi1x_0x).
+ssl_call (len1x, lo1x, hi1x, a1).
+exists (h_sll_nxtx1len1xlo1xhi1x_0x);
 sslauto.
 ssl_frame_unfold.
 move=>h_call0.
-ex_elim h_sll_nxtx2len1xlo1xhi1x_5151.
+ex_elim h_sll_nxtx1len1xlo1xhi1x_21.
 move=>[sigma_call0].
 subst h_call0.
-move=>H_sll_nxtx2len1xlo1xhi1x_5151.
+move=>H_sll_nxtx1len1xlo1xhi1x_21.
 store_valid.
 ssl_read r.
-try rename lo1x into lo1x2.
-try rename h_sll_xlen1xvx2lo1xvx2lo1xhi1xvx2vx2hi1x_515 into h_sll_xlen1xvx2lo1x2vx2lo1x2hi1xvx2vx2hi1x_515.
-try rename H_sll_xlen1xvx2lo1xvx2lo1xhi1xvx2vx2hi1x_515 into H_sll_xlen1xvx2lo1x2vx2lo1x2hi1xvx2vx2hi1x_515.
-try rename h_sll_nxtx2len1xlo1xhi1x_513x into h_sll_nxtx2len1xlo1x2hi1x_513x.
-try rename H_sll_nxtx2len1xlo1xhi1x_513x into H_sll_nxtx2len1xlo1x2hi1x_513x.
-try rename h_sll_nxtx2len1xlo1xhi1x_5151 into h_sll_nxtx2len1xlo1x2hi1x_5151.
-try rename H_sll_nxtx2len1xlo1xhi1x_5151 into H_sll_nxtx2len1xlo1x2hi1x_5151.
-try rename h_sll_xlen1xvx2lo1xvx2lo1xhi1xvx2vx2hi1x_514 into h_sll_xlen1xvx2lo1x2vx2lo1x2hi1xvx2vx2hi1x_514.
-try rename H_sll_xlen1xvx2lo1xvx2lo1xhi1xvx2vx2hi1x_514 into H_sll_xlen1xvx2lo1x2vx2lo1x2hi1xvx2vx2hi1x_514.
-try rename h_sll_nxtx1len1x1lo11xhi11x_513x1 into h_sll_nxtx2len1xlo1x2hi1x_5151.
-try rename H_sll_nxtx1len1x1lo11xhi11x_513x1 into H_sll_nxtx2len1xlo1x2hi1x_5151.
+try rename lo1x into lo1x1.
+try rename h_sll_xlen1xvx1lo1xvx1lo1xhi1xvx1vx1hi1x_1 into h_sll_xlen1xvx1lo1x1vx1lo1x1hi1xvx1vx1hi1x_1.
+try rename H_sll_xlen1xvx1lo1xvx1lo1xhi1xvx1vx1hi1x_1 into H_sll_xlen1xvx1lo1x1vx1lo1x1hi1xvx1vx1hi1x_1.
+try rename h_sll_nxtx1len1xlo1xhi1x_21 into h_sll_nxtx1len1xlo1x1hi1x_21.
+try rename H_sll_nxtx1len1xlo1xhi1x_21 into H_sll_nxtx1len1xlo1x1hi1x_21.
+try rename h_sll_nxtx1len1xlo1xhi1x_0x into h_sll_nxtx1len1xlo1x1hi1x_0x.
+try rename H_sll_nxtx1len1xlo1xhi1x_0x into H_sll_nxtx1len1xlo1x1hi1x_0x.
+try rename h_sll_xlen1xvx1lo1xvx1lo1xhi1xvx1vx1hi1x_2 into h_sll_xlen1xvx1lo1x1vx1lo1x1hi1xvx1vx1hi1x_2.
+try rename H_sll_xlen1xvx1lo1xvx1lo1xhi1xvx1vx1hi1x_2 into H_sll_xlen1xvx1lo1x1vx1lo1x1hi1xvx1vx1hi1x_2.
+try rename h_sll_nxtx2len1x1lo11xhi11x_0x1 into h_sll_nxtx1len1xlo1x1hi1x_21.
+try rename H_sll_nxtx2len1x1lo11xhi11x_0x1 into H_sll_nxtx1len1xlo1x1hi1x_21.
 ssl_write r.
 ssl_write_post r.
 ssl_emp;
-exists (x :-> vx2 \+ x .+ 1 :-> nxtx2 \+ h_sll_nxtx2len1xlo1x2hi1x_5151);
+exists (x :-> (vx1) \+ x .+ 1 :-> (nxtx1) \+ h_sll_nxtx1len1xlo1x1hi1x_21);
 sslauto.
 ssl_close 2;
-exists (len1x), (vx2), (hi1x), (lo1x2), (nxtx2), (h_sll_nxtx2len1xlo1x2hi1x_5151);
+exists (len1x), (vx1), (hi1x), (lo1x1), (nxtx1), (h_sll_nxtx1len1xlo1x1hi1x_21);
 sslauto.
 ssl_frame_unfold.
 Qed.
