benchmarks/standard/sll/sll_append.v
@@ -8,6 +8,7 @@ From SSL
 Require Import core.
 From Hammer Require Import Hammer.
 (* Configure Hammer *)
+Set Hammer ATPLimit 60.
 Unset Hammer Eprover.
 Unset Hammer Vampire.
 Add Search Blacklist "fcsl.".
@@ -25,8 +26,8 @@ Add Search Blacklist "mathcomp.ssreflect.tuple".
 
 Require Import common.
 
-Lemma pure27 (vx12 : nat) (s1x1 : seq nat) (s2 : seq nat) : ((([:: vx12]) ++ (s1x1)) ++ (s2)) = (([:: vx12]) ++ ((s1x1) ++ (s2))). intros; hammer. Qed.
-Hint Resolve pure27: ssl_pure.
+Lemma pure1 (vx11 : nat) (s1x1 : seq nat) (s2 : seq nat) : ((([:: vx11]) ++ (s1x1)) ++ (s2)) = (([:: vx11]) ++ ((s1x1) ++ (s2))). intros; hammer. Qed.
+Hint Resolve pure1: ssl_pure.
 
 Definition sll_append_type :=
   forall (vprogs : ptr * ptr),
@@ -35,121 +36,121 @@ Definition sll_append_type :=
     fun h =>
       let: (x1, r) := vprogs in
       let: (s1, x2, s2) := vghosts in
-      exists h_sll_x1s1_528 h_sll_x2s2_529,
-      h = r :-> x2 \+ h_sll_x1s1_528 \+ h_sll_x2s2_529 /\ sll x1 s1 h_sll_x1s1_528 /\ sll x2 s2 h_sll_x2s2_529,
+      exists h_sll_x1s1_1 h_sll_x2s2_2,
+      h = r :-> (x2) \+ h_sll_x1s1_1 \+ h_sll_x2s2_2 /\ sll x1 s1 h_sll_x1s1_1 /\ sll x2 s2 h_sll_x2s2_2,
     [vfun (_: unit) h =>
       let: (x1, r) := vprogs in
       let: (s1, x2, s2) := vghosts in
       exists s y,
-      exists h_sll_ys_530,
-      (s) == ((s1) ++ (s2)) /\ h = r :-> y \+ h_sll_ys_530 /\ sll y s h_sll_ys_530
+      exists h_sll_ys_3,
+      (s) == ((s1) ++ (s2)) /\ h = r :-> (y) \+ h_sll_ys_3 /\ sll y s h_sll_ys_3
     ]).
 
 Program Definition sll_append : sll_append_type :=
   Fix (fun (sll_append : sll_append_type) vprogs =>
     let: (x1, r) := vprogs in
     Do (
-      x22 <-- @read ptr r;
+      x21 <-- @read ptr r;
       if (x1) == (null)
       then
         ret tt
       else
-        vx12 <-- @read nat x1;
-        nxtx12 <-- @read ptr (x1 .+ 1);
-        sll_append (nxtx12, r);;
-        y12 <-- @read ptr r;
-        (x1 .+ 1) ::= y12;;
+        vx11 <-- @read nat x1;
+        nxtx11 <-- @read ptr (x1 .+ 1);
+        sll_append (nxtx11, r);;
+        y11 <-- @read ptr r;
         r ::= x1;;
+        (x1 .+ 1) ::= y11;;
         ret tt
     )).
 Obligation Tactic := intro; move=>[x1 r]; ssl_program_simpl.
 Next Obligation.
 ssl_ghostelim_pre.
 move=>[[s1 x2] s2].
-ex_elim h_sll_x1s1_528 h_sll_x2s2_529.
+ex_elim h_sll_x1s1_1 h_sll_x2s2_2.
 move=>[sigma_self].
 subst h_self.
-move=>[H_sll_x1s1_528 H_sll_x2s2_529].
+move=>[H_sll_x1s1_1 H_sll_x2s2_2].
 ssl_ghostelim_post.
-try rename h_sll_ys_530 into h_sll_ys1s2_530.
-try rename H_sll_ys_530 into H_sll_ys1s2_530.
+try rename h_sll_ys_3 into h_sll_ys1s2_3.
+try rename H_sll_ys_3 into H_sll_ys1s2_3.
 ssl_read r.
-try rename x2 into x22.
-try rename h_sll_x2s2_529 into h_sll_x22s2_529.
-try rename H_sll_x2s2_529 into H_sll_x22s2_529.
-ssl_open ((x1) == (null)) H_sll_x1s1_528.
-move=>[phi_sll_x1s1_5280].
-move=>[sigma_sll_x1s1_528].
-subst h_sll_x1s1_528.
-try rename h_sll_x1s1_528 into h_sll_x1_528.
-try rename H_sll_x1s1_528 into H_sll_x1_528.
-try rename h_sll_ys1s2_530 into h_sll_ys2_530.
-try rename H_sll_ys1s2_530 into H_sll_ys2_530.
-try rename h_sll_ys2_530 into h_sll_x22s2_529.
-try rename H_sll_ys2_530 into H_sll_x22s2_529.
+try rename x2 into x21.
+try rename h_sll_x2s2_2 into h_sll_x21s2_2.
+try rename H_sll_x2s2_2 into H_sll_x21s2_2.
+ssl_open ((x1) == (null)) H_sll_x1s1_1.
+move=>[phi_sll_x1s1_10].
+move=>[sigma_sll_x1s1_1].
+subst h_sll_x1s1_1.
+try rename h_sll_x1s1_1 into h_sll_x1_1.
+try rename H_sll_x1s1_1 into H_sll_x1_1.
+try rename h_sll_ys1s2_3 into h_sll_ys2_3.
+try rename H_sll_ys1s2_3 into H_sll_ys2_3.
+try rename h_sll_ys2_3 into h_sll_x21s2_2.
+try rename H_sll_ys2_3 into H_sll_x21s2_2.
 ssl_emp;
-exists (s2), (x22);
-exists (h_sll_x22s2_529);
+exists (s2), (x21);
+exists (h_sll_x21s2_2);
 sslauto.
 ssl_frame_unfold.
 ex_elim vx1 s1x1 nxtx1.
-ex_elim h_sll_nxtx1s1x1_527x1.
-move=>[phi_sll_x1s1_5280].
-move=>[sigma_sll_x1s1_528].
-subst h_sll_x1s1_528.
-move=>H_sll_nxtx1s1x1_527x1.
-try rename h_sll_x1s1_528 into h_sll_x1vx1s1x1_528.
-try rename H_sll_x1s1_528 into H_sll_x1vx1s1x1_528.
-try rename h_sll_ys1s2_530 into h_sll_yvx1s1x1s2_530.
-try rename H_sll_ys1s2_530 into H_sll_yvx1s1x1s2_530.
+ex_elim h_sll_nxtx1s1x1_0x1.
+move=>[phi_sll_x1s1_10].
+move=>[sigma_sll_x1s1_1].
+subst h_sll_x1s1_1.
+move=>H_sll_nxtx1s1x1_0x1.
+try rename h_sll_x1s1_1 into h_sll_x1vx1s1x1_1.
+try rename H_sll_x1s1_1 into H_sll_x1vx1s1x1_1.
+try rename h_sll_ys1s2_3 into h_sll_yvx1s1x1s2_3.
+try rename H_sll_ys1s2_3 into H_sll_yvx1s1x1s2_3.
 ssl_read x1.
-try rename vx1 into vx12.
-try rename h_sll_yvx1s1x1s2_530 into h_sll_yvx12s1x1s2_530.
-try rename H_sll_yvx1s1x1s2_530 into H_sll_yvx12s1x1s2_530.
-try rename h_sll_x1vx1s1x1_528 into h_sll_x1vx12s1x1_528.
-try rename H_sll_x1vx1s1x1_528 into H_sll_x1vx12s1x1_528.
+try rename vx1 into vx11.
+try rename h_sll_yvx1s1x1s2_3 into h_sll_yvx11s1x1s2_3.
+try rename H_sll_yvx1s1x1s2_3 into H_sll_yvx11s1x1s2_3.
+try rename h_sll_x1vx1s1x1_1 into h_sll_x1vx11s1x1_1.
+try rename H_sll_x1vx1s1x1_1 into H_sll_x1vx11s1x1_1.
 ssl_read (x1 .+ 1).
-try rename nxtx1 into nxtx12.
-try rename h_sll_nxtx1s1x1_527x1 into h_sll_nxtx12s1x1_527x1.
-try rename H_sll_nxtx1s1x1_527x1 into H_sll_nxtx12s1x1_527x1.
-try rename h_sll_x11s11_5281 into h_sll_nxtx12s1x1_527x1.
-try rename H_sll_x11s11_5281 into H_sll_nxtx12s1x1_527x1.
-try rename h_sll_x21s21_5291 into h_sll_x22s2_529.
-try rename H_sll_x21s21_5291 into H_sll_x22s2_529.
-ssl_call_pre (r :-> x22 \+ h_sll_nxtx12s1x1_527x1 \+ h_sll_x22s2_529).
-ssl_call (s1x1, x22, s2).
-exists (h_sll_nxtx12s1x1_527x1), (h_sll_x22s2_529);
+try rename nxtx1 into nxtx11.
+try rename h_sll_nxtx1s1x1_0x1 into h_sll_nxtx11s1x1_0x1.
+try rename H_sll_nxtx1s1x1_0x1 into H_sll_nxtx11s1x1_0x1.
+try rename h_sll_x11s11_11 into h_sll_nxtx11s1x1_0x1.
+try rename H_sll_x11s11_11 into H_sll_nxtx11s1x1_0x1.
+try rename h_sll_x22s21_21 into h_sll_x21s2_2.
+try rename H_sll_x22s21_21 into H_sll_x21s2_2.
+ssl_call_pre (r :-> (x21) \+ h_sll_nxtx11s1x1_0x1 \+ h_sll_x21s2_2).
+ssl_call (s1x1, x21, s2).
+exists (h_sll_nxtx11s1x1_0x1), (h_sll_x21s2_2);
 sslauto.
 ssl_frame_unfold.
 ssl_frame_unfold.
 move=>h_call0.
 ex_elim s3 y1.
-ex_elim h_sll_y1s3_5301.
+ex_elim h_sll_y1s3_31.
 move=>[phi_call00].
 move=>[sigma_call0].
 subst h_call0.
-move=>H_sll_y1s3_5301.
+move=>H_sll_y1s3_31.
 store_valid.
-try rename h_sll_y1s3_5301 into h_sll_y1s1x1s2_5301.
-try rename H_sll_y1s3_5301 into H_sll_y1s1x1s2_5301.
+try rename h_sll_y1s3_31 into h_sll_y1s1x1s2_31.
+try rename H_sll_y1s3_31 into H_sll_y1s1x1s2_31.
 ssl_read r.
-try rename y1 into y12.
-try rename h_sll_y1s1x1s2_5301 into h_sll_y12s1x1s2_5301.
-try rename H_sll_y1s1x1s2_5301 into H_sll_y12s1x1s2_5301.
-try rename h_sll_nxtys12y_527y into h_sll_y12s1x1s2_5301.
-try rename H_sll_nxtys12y_527y into H_sll_y12s1x1s2_5301.
-try rename h_sll_yvx12s1x1s2_530 into h_sll_x1vx12s1x1s2_530.
-try rename H_sll_yvx12s1x1s2_530 into H_sll_x1vx12s1x1s2_530.
-ssl_write (x1 .+ 1).
-ssl_write_post (x1 .+ 1).
+try rename y1 into y11.
+try rename h_sll_y1s1x1s2_31 into h_sll_y11s1x1s2_31.
+try rename H_sll_y1s1x1s2_31 into H_sll_y11s1x1s2_31.
+try rename h_sll_nxtys12y_0y into h_sll_y11s1x1s2_31.
+try rename H_sll_nxtys12y_0y into H_sll_y11s1x1s2_31.
+try rename h_sll_yvx11s1x1s2_3 into h_sll_x1vx11s1x1s2_3.
+try rename H_sll_yvx11s1x1s2_3 into H_sll_x1vx11s1x1s2_3.
 ssl_write r.
 ssl_write_post r.
+ssl_write (x1 .+ 1).
+ssl_write_post (x1 .+ 1).
 ssl_emp;
-exists ((([:: vx12]) ++ (s1x1)) ++ (s2)), (x1);
-exists (x1 :-> vx12 \+ x1 .+ 1 :-> y12 \+ h_sll_y12s1x1s2_5301);
+exists ((([:: vx11]) ++ (s1x1)) ++ (s2)), (x1);
+exists (x1 :-> (vx11) \+ x1 .+ 1 :-> (y11) \+ h_sll_y11s1x1s2_31);
 sslauto.
 ssl_close 2;
-exists (vx12), ((s1x1) ++ (s2)), (y12), (h_sll_y12s1x1s2_5301);
+exists (vx11), ((s1x1) ++ (s2)), (y11), (h_sll_y11s1x1s2_31);
 sslauto.
 ssl_frame_unfold.
 Qed.
