benchmarks/standard/sll/sll_copy.v
@@ -8,6 +8,7 @@ From SSL
 Require Import core.
 From Hammer Require Import Hammer.
 (* Configure Hammer *)
+Set Hammer ATPLimit 60.
 Unset Hammer Eprover.
 Unset Hammer Vampire.
 Add Search Blacklist "fcsl.".
@@ -25,14 +26,14 @@ Add Search Blacklist "mathcomp.ssreflect.tuple".
 
 Require Import common.
 
-Lemma pure23 : (@nil nat) = (@nil nat). intros; hammer. Qed.
-Hint Resolve pure23: ssl_pure.
-Lemma pure24 (b1 : nat) : (b1) < ((b1) + (1)). intros; hammer. Qed.
-Hint Resolve pure24: ssl_pure.
-Lemma pure25 (vx22 : nat) (s1x2 : seq nat) : (([:: vx22]) ++ (s1x2)) = (([:: vx22]) ++ (s1x2)). intros; hammer. Qed.
-Hint Resolve pure25: ssl_pure.
-Lemma pure26 (vx22 : nat) (s1x2 : seq nat) : (([:: vx22]) ++ (s1x2)) = (([:: vx22]) ++ (s1x2)). intros; hammer. Qed.
-Hint Resolve pure26: ssl_pure.
+Lemma pure1 : (@nil nat) = (@nil nat). intros; hammer. Qed.
+Hint Resolve pure1: ssl_pure.
+Lemma pure2 (b1 : nat) : (b1) < ((b1) + (1)). intros; hammer. Qed.
+Hint Resolve pure2: ssl_pure.
+Lemma pure3 (vx11 : nat) (s1x1 : seq nat) : (([:: vx11]) ++ (s1x1)) = (([:: vx11]) ++ (s1x1)). intros; hammer. Qed.
+Hint Resolve pure3: ssl_pure.
+Lemma pure4 (vx11 : nat) (s1x1 : seq nat) : (([:: vx11]) ++ (s1x1)) = (([:: vx11]) ++ (s1x1)). intros; hammer. Qed.
+Hint Resolve pure4: ssl_pure.
 
 Definition sll_copy_type :=
   forall (vprogs : ptr),
@@ -42,33 +43,33 @@ Definition sll_copy_type :=
       let: (r) := vprogs in
       let: (x, s) := vghosts in
       exists h_sll_xs_a,
-      h = r :-> x \+ h_sll_xs_a /\ sll x s h_sll_xs_a,
+      h = r :-> (x) \+ h_sll_xs_a /\ sll x s h_sll_xs_a,
     [vfun (_: unit) h =>
       let: (r) := vprogs in
       let: (x, s) := vghosts in
       exists y,
       exists h_sll_xs_a h_sll_ys_b,
-      h = r :-> y \+ h_sll_xs_a \+ h_sll_ys_b /\ sll x s h_sll_xs_a /\ sll y s h_sll_ys_b
+      h = r :-> (y) \+ h_sll_xs_a \+ h_sll_ys_b /\ sll x s h_sll_xs_a /\ sll y s h_sll_ys_b
     ]).
 
 Program Definition sll_copy : sll_copy_type :=
   Fix (fun (sll_copy : sll_copy_type) vprogs =>
     let: (r) := vprogs in
     Do (
-      x2 <-- @read ptr r;
-      if (x2) == (null)
+      x1 <-- @read ptr r;
+      if (x1) == (null)
       then
         ret tt
       else
-        vx22 <-- @read nat x2;
-        nxtx22 <-- @read ptr (x2 .+ 1);
-        r ::= nxtx22;;
+        vx11 <-- @read nat x1;
+        nxtx11 <-- @read ptr (x1 .+ 1);
+        r ::= nxtx11;;
         sll_copy (r);;
-        y12 <-- @read ptr r;
+        y11 <-- @read ptr r;
         y2 <-- allocb null 2;
         r ::= y2;;
-        (y2 .+ 1) ::= y12;;
-        y2 ::= vx22;;
+        (y2 .+ 1) ::= y11;;
+        y2 ::= vx11;;
         ret tt
     )).
 Obligation Tactic := intro; move=>r; ssl_program_simpl.
@@ -81,17 +82,17 @@ subst h_self.
 move=>H_sll_xs_a.
 ssl_ghostelim_post.
 ssl_read r.
-try rename x into x2.
-try rename h_sll_xs_a into h_sll_x2s_a.
-try rename H_sll_xs_a into H_sll_x2s_a.
-ssl_open ((x2) == (null)) H_sll_x2s_a.
-move=>[phi_sll_x2s_a0].
-move=>[sigma_sll_x2s_a].
-subst h_sll_x2s_a.
+try rename x into x1.
+try rename h_sll_xs_a into h_sll_x1s_a.
+try rename H_sll_xs_a into H_sll_x1s_a.
+ssl_open ((x1) == (null)) H_sll_x1s_a.
+move=>[phi_sll_x1s_a0].
+move=>[sigma_sll_x1s_a].
+subst h_sll_x1s_a.
 try rename h_sll_ys_b into h_sll_y_b.
 try rename H_sll_ys_b into H_sll_y_b.
-try rename h_sll_x2s_a into h_sll_x2_a.
-try rename H_sll_x2s_a into H_sll_x2_a.
+try rename h_sll_x1s_a into h_sll_x1_a.
+try rename H_sll_x1s_a into H_sll_x1_a.
 try rename h_sll_y_b into h_sll__b.
 try rename H_sll_y_b into H_sll__b.
 ssl_emp;
@@ -103,53 +104,53 @@ ssl_close 1;
 sslauto.
 ssl_close 1;
 sslauto.
-ex_elim vx2 s1x2 nxtx2.
-ex_elim h_sll_nxtx2s1x2_524x2.
-move=>[phi_sll_x2s_a0].
-move=>[sigma_sll_x2s_a].
-subst h_sll_x2s_a.
-move=>H_sll_nxtx2s1x2_524x2.
-try rename h_sll_ys_b into h_sll_yvx2s1x2_b.
-try rename H_sll_ys_b into H_sll_yvx2s1x2_b.
-try rename h_sll_x2s_a into h_sll_x2vx2s1x2_a.
-try rename H_sll_x2s_a into H_sll_x2vx2s1x2_a.
-ssl_read x2.
-try rename vx2 into vx22.
-try rename h_sll_yvx2s1x2_b into h_sll_yvx22s1x2_b.
-try rename H_sll_yvx2s1x2_b into H_sll_yvx22s1x2_b.
-try rename h_sll_x2vx2s1x2_a into h_sll_x2vx22s1x2_a.
-try rename H_sll_x2vx2s1x2_a into H_sll_x2vx22s1x2_a.
-ssl_read (x2 .+ 1).
-try rename nxtx2 into nxtx22.
-try rename h_sll_nxtx2s1x2_524x2 into h_sll_nxtx22s1x2_524x2.
-try rename H_sll_nxtx2s1x2_524x2 into H_sll_nxtx22s1x2_524x2.
-try rename h_sll_x1s1_a1 into h_sll_nxtx22s1x2_524x2.
-try rename H_sll_x1s1_a1 into H_sll_nxtx22s1x2_524x2.
+ex_elim vx1 s1x1 nxtx1.
+ex_elim h_sll_nxtx1s1x1_0x1.
+move=>[phi_sll_x1s_a0].
+move=>[sigma_sll_x1s_a].
+subst h_sll_x1s_a.
+move=>H_sll_nxtx1s1x1_0x1.
+try rename h_sll_ys_b into h_sll_yvx1s1x1_b.
+try rename H_sll_ys_b into H_sll_yvx1s1x1_b.
+try rename h_sll_x1s_a into h_sll_x1vx1s1x1_a.
+try rename H_sll_x1s_a into H_sll_x1vx1s1x1_a.
+ssl_read x1.
+try rename vx1 into vx11.
+try rename h_sll_yvx1s1x1_b into h_sll_yvx11s1x1_b.
+try rename H_sll_yvx1s1x1_b into H_sll_yvx11s1x1_b.
+try rename h_sll_x1vx1s1x1_a into h_sll_x1vx11s1x1_a.
+try rename H_sll_x1vx1s1x1_a into H_sll_x1vx11s1x1_a.
+ssl_read (x1 .+ 1).
+try rename nxtx1 into nxtx11.
+try rename h_sll_nxtx1s1x1_0x1 into h_sll_nxtx11s1x1_0x1.
+try rename H_sll_nxtx1s1x1_0x1 into H_sll_nxtx11s1x1_0x1.
+try rename h_sll_x2s1_a1 into h_sll_nxtx11s1x1_0x1.
+try rename H_sll_x2s1_a1 into H_sll_nxtx11s1x1_0x1.
 ssl_write r.
-ssl_call_pre (r :-> nxtx22 \+ h_sll_nxtx22s1x2_524x2).
-ssl_call (nxtx22, s1x2).
-exists (h_sll_nxtx22s1x2_524x2);
+ssl_call_pre (r :-> (nxtx11) \+ h_sll_nxtx11s1x1_0x1).
+ssl_call (nxtx11, s1x1).
+exists (h_sll_nxtx11s1x1_0x1);
 sslauto.
 ssl_frame_unfold.
 move=>h_call0.
 ex_elim y1.
-ex_elim h_sll_nxtx22s1x2_524x2 h_sll_y1s1x2_b1.
+ex_elim h_sll_nxtx11s1x1_0x1 h_sll_y1s1x1_b1.
 move=>[sigma_call0].
 subst h_call0.
-move=>[H_sll_nxtx22s1x2_524x2 H_sll_y1s1x2_b1].
+move=>[H_sll_nxtx11s1x1_0x1 H_sll_y1s1x1_b1].
 store_valid.
 ssl_read r.
-try rename y1 into y12.
-try rename h_sll_y1s1x2_b1 into h_sll_y12s1x2_b1.
-try rename H_sll_y1s1x2_b1 into H_sll_y12s1x2_b1.
-try rename h_sll_nxtx21s11x2_524x21 into h_sll_nxtx22s1x2_524x2.
-try rename H_sll_nxtx21s11x2_524x21 into H_sll_nxtx22s1x2_524x2.
-try rename h_sll_nxtys11y_524y into h_sll_y12s1x2_b1.
-try rename H_sll_nxtys11y_524y into H_sll_y12s1x2_b1.
+try rename y1 into y11.
+try rename h_sll_y1s1x1_b1 into h_sll_y11s1x1_b1.
+try rename H_sll_y1s1x1_b1 into H_sll_y11s1x1_b1.
+try rename h_sll_nxtx12s11x1_0x11 into h_sll_nxtx11s1x1_0x1.
+try rename H_sll_nxtx12s11x1_0x11 into H_sll_nxtx11s1x1_0x1.
+try rename h_sll_nxtys11y_0y into h_sll_y11s1x1_b1.
+try rename H_sll_nxtys11y_0y into H_sll_y11s1x1_b1.
 ssl_alloc y2.
 try rename y into y2.
-try rename h_sll_yvx22s1x2_b into h_sll_y2vx22s1x2_b.
-try rename H_sll_yvx22s1x2_b into H_sll_y2vx22s1x2_b.
+try rename h_sll_yvx11s1x1_b into h_sll_y2vx11s1x1_b.
+try rename H_sll_yvx11s1x1_b into H_sll_y2vx11s1x1_b.
 ssl_write r.
 ssl_write_post r.
 ssl_write (y2 .+ 1).
@@ -158,15 +159,15 @@ ssl_write y2.
 ssl_write_post y2.
 ssl_emp;
 exists (y2);
-exists (x2 :-> vx22 \+ x2 .+ 1 :-> nxtx22 \+ h_sll_nxtx22s1x2_524x2);
-exists (y2 :-> vx22 \+ y2 .+ 1 :-> y12 \+ h_sll_y12s1x2_b1);
+exists (x1 :-> (vx11) \+ x1 .+ 1 :-> (nxtx11) \+ h_sll_nxtx11s1x1_0x1);
+exists (y2 :-> (vx11) \+ y2 .+ 1 :-> (y11) \+ h_sll_y11s1x1_b1);
 sslauto.
 ssl_close 2;
-exists (vx22), (s1x2), (nxtx22), (h_sll_nxtx22s1x2_524x2);
+exists (vx11), (s1x1), (nxtx11), (h_sll_nxtx11s1x1_0x1);
 sslauto.
 shelve.
 ssl_close 2;
-exists (vx22), (s1x2), (y12), (h_sll_y12s1x2_b1);
+exists (vx11), (s1x1), (y11), (h_sll_y11s1x1_b1);
 sslauto.
 shelve.
 Unshelve.
