benchmarks/standard/sll/sll_free.v
@@ -8,6 +8,7 @@ From SSL
 Require Import core.
 From Hammer Require Import Hammer.
 (* Configure Hammer *)
+Set Hammer ATPLimit 60.
 Unset Hammer Eprover.
 Unset Hammer Vampire.
 Add Search Blacklist "fcsl.".
@@ -32,8 +33,8 @@ Definition sll_free_type :=
     fun h =>
       let: (x) := vprogs in
       let: (s) := vghosts in
-      exists h_sll_xs_526,
-      h = h_sll_xs_526 /\ sll x s h_sll_xs_526,
+      exists h_sll_xs_1,
+      h = h_sll_xs_1 /\ sll x s h_sll_xs_1,
     [vfun (_: unit) h =>
       let: (x) := vprogs in
       let: (s) := vghosts in
@@ -48,9 +49,9 @@ Program Definition sll_free : sll_free_type :=
       then
         ret tt
       else
-        vx2 <-- @read nat x;
-        nxtx2 <-- @read ptr (x .+ 1);
-        sll_free (nxtx2);;
+        vx1 <-- @read nat x;
+        nxtx1 <-- @read ptr (x .+ 1);
+        sll_free (nxtx1);;
         dealloc x;;
         dealloc (x .+ 1);;
         ret tt
@@ -59,40 +60,40 @@ Obligation Tactic := intro; move=>x; ssl_program_simpl.
 Next Obligation.
 ssl_ghostelim_pre.
 move=>s.
-ex_elim h_sll_xs_526.
+ex_elim h_sll_xs_1.
 move=>[sigma_self].
 subst h_self.
-move=>H_sll_xs_526.
+move=>H_sll_xs_1.
 ssl_ghostelim_post.
-ssl_open ((x) == (null)) H_sll_xs_526.
-move=>[phi_sll_xs_5260].
-move=>[sigma_sll_xs_526].
-subst h_sll_xs_526.
-try rename h_sll_xs_526 into h_sll_x_526.
-try rename H_sll_xs_526 into H_sll_x_526.
+ssl_open ((x) == (null)) H_sll_xs_1.
+move=>[phi_sll_xs_10].
+move=>[sigma_sll_xs_1].
+subst h_sll_xs_1.
+try rename h_sll_xs_1 into h_sll_x_1.
+try rename H_sll_xs_1 into H_sll_x_1.
 ssl_emp;
 sslauto.
 ex_elim vx s1x nxtx.
-ex_elim h_sll_nxtxs1x_525x.
-move=>[phi_sll_xs_5260].
-move=>[sigma_sll_xs_526].
-subst h_sll_xs_526.
-move=>H_sll_nxtxs1x_525x.
-try rename h_sll_xs_526 into h_sll_xvxs1x_526.
-try rename H_sll_xs_526 into H_sll_xvxs1x_526.
+ex_elim h_sll_nxtxs1x_0x.
+move=>[phi_sll_xs_10].
+move=>[sigma_sll_xs_1].
+subst h_sll_xs_1.
+move=>H_sll_nxtxs1x_0x.
+try rename h_sll_xs_1 into h_sll_xvxs1x_1.
+try rename H_sll_xs_1 into H_sll_xvxs1x_1.
 ssl_read x.
-try rename vx into vx2.
-try rename h_sll_xvxs1x_526 into h_sll_xvx2s1x_526.
-try rename H_sll_xvxs1x_526 into H_sll_xvx2s1x_526.
+try rename vx into vx1.
+try rename h_sll_xvxs1x_1 into h_sll_xvx1s1x_1.
+try rename H_sll_xvxs1x_1 into H_sll_xvx1s1x_1.
 ssl_read (x .+ 1).
-try rename nxtx into nxtx2.
-try rename h_sll_nxtxs1x_525x into h_sll_nxtx2s1x_525x.
-try rename H_sll_nxtxs1x_525x into H_sll_nxtx2s1x_525x.
-try rename h_sll_x1s1_5261 into h_sll_nxtx2s1x_525x.
-try rename H_sll_x1s1_5261 into H_sll_nxtx2s1x_525x.
-ssl_call_pre (h_sll_nxtx2s1x_525x).
+try rename nxtx into nxtx1.
+try rename h_sll_nxtxs1x_0x into h_sll_nxtx1s1x_0x.
+try rename H_sll_nxtxs1x_0x into H_sll_nxtx1s1x_0x.
+try rename h_sll_x1s1_11 into h_sll_nxtx1s1x_0x.
+try rename H_sll_x1s1_11 into H_sll_nxtx1s1x_0x.
+ssl_call_pre (h_sll_nxtx1s1x_0x).
 ssl_call (s1x).
-exists (h_sll_nxtx2s1x_525x);
+exists (h_sll_nxtx1s1x_0x);
 sslauto.
 ssl_frame_unfold.
 move=>h_call0.
