benchmarks/standard/sll/sll_singleton.v
@@ -8,6 +8,7 @@ From SSL
 Require Import core.
 From Hammer Require Import Hammer.
 (* Configure Hammer *)
+Set Hammer ATPLimit 60.
 Unset Hammer Eprover.
 Unset Hammer Vampire.
 Add Search Blacklist "fcsl.".
@@ -25,8 +26,8 @@ Add Search Blacklist "mathcomp.ssreflect.tuple".
 
 Require Import common.
 
-Lemma pure28 (x : nat) : ([:: x]) = ([:: x]). intros; hammer. Qed.
-Hint Resolve pure28: ssl_pure.
+Lemma pure1 (x : nat) : ([:: x]) = ([:: x]). intros; hammer. Qed.
+Hint Resolve pure1: ssl_pure.
 
 Definition sll_singleton_type :=
   forall (vprogs : nat * ptr),
@@ -35,24 +36,24 @@ Definition sll_singleton_type :=
     fun h =>
       let: (x, p) := vprogs in
       let: (a) := vghosts in
-      h = p :-> a,
+      h = p :-> (a),
     [vfun (_: unit) h =>
       let: (x, p) := vprogs in
       let: (a) := vghosts in
       exists elems y,
-      exists h_sll_yelems_532,
-      (elems) == ([:: x]) /\ h = p :-> y \+ h_sll_yelems_532 /\ sll y elems h_sll_yelems_532
+      exists h_sll_yelems_1,
+      (elems) == ([:: x]) /\ h = p :-> (y) \+ h_sll_yelems_1 /\ sll y elems h_sll_yelems_1
     ]).
 
 Program Definition sll_singleton : sll_singleton_type :=
   Fix (fun (sll_singleton : sll_singleton_type) vprogs =>
     let: (x, p) := vprogs in
     Do (
-      a2 <-- @read ptr p;
-      y2 <-- allocb null 2;
-      p ::= y2;;
-      (y2 .+ 1) ::= null;;
-      y2 ::= x;;
+      a1 <-- @read ptr p;
+      y1 <-- allocb null 2;
+      p ::= y1;;
+      (y1 .+ 1) ::= null;;
+      y1 ::= x;;
       ret tt
     )).
 Obligation Tactic := intro; move=>[x p]; ssl_program_simpl.
@@ -62,27 +63,27 @@ move=>a.
 move=>[sigma_self].
 subst h_self.
 ssl_ghostelim_post.
-try rename h_sll_yelems_532 into h_sll_yx_532.
-try rename H_sll_yelems_532 into H_sll_yx_532.
+try rename h_sll_yelems_1 into h_sll_yx_1.
+try rename H_sll_yelems_1 into H_sll_yx_1.
 ssl_read p.
-try rename a into a2.
-try rename h_sll_nxtys1y_531y into h_sll_s1y_531y.
-try rename H_sll_nxtys1y_531y into H_sll_s1y_531y.
-try rename h_sll_s1y_531y into h_sll__531y.
-try rename H_sll_s1y_531y into H_sll__531y.
-ssl_alloc y2.
-try rename y into y2.
-try rename h_sll_yx_532 into h_sll_y2x_532.
-try rename H_sll_yx_532 into H_sll_y2x_532.
+try rename a into a1.
+try rename h_sll_nxtys1y_0y into h_sll_s1y_0y.
+try rename H_sll_nxtys1y_0y into H_sll_s1y_0y.
+try rename h_sll_s1y_0y into h_sll__0y.
+try rename H_sll_s1y_0y into H_sll__0y.
+ssl_alloc y1.
+try rename y into y1.
+try rename h_sll_yx_1 into h_sll_y1x_1.
+try rename H_sll_yx_1 into H_sll_y1x_1.
 ssl_write p.
 ssl_write_post p.
-ssl_write (y2 .+ 1).
-ssl_write_post (y2 .+ 1).
-ssl_write y2.
-ssl_write_post y2.
+ssl_write (y1 .+ 1).
+ssl_write_post (y1 .+ 1).
+ssl_write y1.
+ssl_write_post y1.
 ssl_emp;
-exists ([:: x]), (y2);
-exists (y2 :-> x \+ y2 .+ 1 :-> null);
+exists ([:: x]), (y1);
+exists (y1 :-> (x) \+ y1 .+ 1 :-> (null));
 sslauto.
 ssl_close 2;
 exists (x), (@nil nat), (null), (empty);
