benchmarks/standard/tree/tree_free.v
@@ -8,6 +8,7 @@ From SSL
 Require Import core.
 From Hammer Require Import Hammer.
 (* Configure Hammer *)
+Set Hammer ATPLimit 60.
 Unset Hammer Eprover.
 Unset Hammer Vampire.
 Add Search Blacklist "fcsl.".
@@ -32,8 +33,8 @@ Definition tree_free_type :=
     fun h =>
       let: (x) := vprogs in
       let: (s) := vghosts in
-      exists h_tree_xs_564,
-      h = h_tree_xs_564 /\ tree x s h_tree_xs_564,
+      exists h_tree_xs_5,
+      h = h_tree_xs_5 /\ tree x s h_tree_xs_5,
     [vfun (_: unit) h =>
       let: (x) := vprogs in
       let: (s) := vghosts in
@@ -48,11 +49,11 @@ Program Definition tree_free : tree_free_type :=
       then
         ret tt
       else
-        vx2 <-- @read nat x;
-        lx2 <-- @read ptr (x .+ 1);
-        rx2 <-- @read ptr (x .+ 2);
-        tree_free (lx2);;
-        tree_free (rx2);;
+        vx1 <-- @read nat x;
+        lx1 <-- @read ptr (x .+ 1);
+        rx1 <-- @read ptr (x .+ 2);
+        tree_free (lx1);;
+        tree_free (rx1);;
         dealloc x;;
         dealloc (x .+ 1);;
         dealloc (x .+ 2);;
@@ -62,55 +63,55 @@ Obligation Tactic := intro; move=>x; ssl_program_simpl.
 Next Obligation.
 ssl_ghostelim_pre.
 move=>s.
-ex_elim h_tree_xs_564.
+ex_elim h_tree_xs_5.
 move=>[sigma_self].
 subst h_self.
-move=>H_tree_xs_564.
+move=>H_tree_xs_5.
 ssl_ghostelim_post.
-ssl_open ((x) == (null)) H_tree_xs_564.
-move=>[phi_tree_xs_5640].
-move=>[sigma_tree_xs_564].
-subst h_tree_xs_564.
-try rename h_tree_xs_564 into h_tree_x_564.
-try rename H_tree_xs_564 into H_tree_x_564.
+ssl_open ((x) == (null)) H_tree_xs_5.
+move=>[phi_tree_xs_50].
+move=>[sigma_tree_xs_5].
+subst h_tree_xs_5.
+try rename h_tree_xs_5 into h_tree_x_5.
+try rename H_tree_xs_5 into H_tree_x_5.
 ssl_emp;
 sslauto.
 ex_elim vx s1x s2x lx rx.
-ex_elim h_tree_lxs1x_559x h_tree_rxs2x_560x.
-move=>[phi_tree_xs_5640].
-move=>[sigma_tree_xs_564].
-subst h_tree_xs_564.
-move=>[H_tree_lxs1x_559x H_tree_rxs2x_560x].
-try rename h_tree_xs_564 into h_tree_xvxs1xs2x_564.
-try rename H_tree_xs_564 into H_tree_xvxs1xs2x_564.
+ex_elim h_tree_lxs1x_0x h_tree_rxs2x_1x.
+move=>[phi_tree_xs_50].
+move=>[sigma_tree_xs_5].
+subst h_tree_xs_5.
+move=>[H_tree_lxs1x_0x H_tree_rxs2x_1x].
+try rename h_tree_xs_5 into h_tree_xvxs1xs2x_5.
+try rename H_tree_xs_5 into H_tree_xvxs1xs2x_5.
 ssl_read x.
-try rename vx into vx2.
-try rename h_tree_xvxs1xs2x_564 into h_tree_xvx2s1xs2x_564.
-try rename H_tree_xvxs1xs2x_564 into H_tree_xvx2s1xs2x_564.
+try rename vx into vx1.
+try rename h_tree_xvxs1xs2x_5 into h_tree_xvx1s1xs2x_5.
+try rename H_tree_xvxs1xs2x_5 into H_tree_xvx1s1xs2x_5.
 ssl_read (x .+ 1).
-try rename lx into lx2.
-try rename h_tree_lxs1x_559x into h_tree_lx2s1x_559x.
-try rename H_tree_lxs1x_559x into H_tree_lx2s1x_559x.
+try rename lx into lx1.
+try rename h_tree_lxs1x_0x into h_tree_lx1s1x_0x.
+try rename H_tree_lxs1x_0x into H_tree_lx1s1x_0x.
 ssl_read (x .+ 2).
-try rename rx into rx2.
-try rename h_tree_rxs2x_560x into h_tree_rx2s2x_560x.
-try rename H_tree_rxs2x_560x into H_tree_rx2s2x_560x.
-try rename h_tree_x1s1_5641 into h_tree_lx2s1x_559x.
-try rename H_tree_x1s1_5641 into H_tree_lx2s1x_559x.
-ssl_call_pre (h_tree_lx2s1x_559x).
+try rename rx into rx1.
+try rename h_tree_rxs2x_1x into h_tree_rx1s2x_1x.
+try rename H_tree_rxs2x_1x into H_tree_rx1s2x_1x.
+try rename h_tree_x1s1_51 into h_tree_lx1s1x_0x.
+try rename H_tree_x1s1_51 into H_tree_lx1s1x_0x.
+ssl_call_pre (h_tree_lx1s1x_0x).
 ssl_call (s1x).
-exists (h_tree_lx2s1x_559x);
+exists (h_tree_lx1s1x_0x);
 sslauto.
 ssl_frame_unfold.
 move=>h_call0.
 move=>[sigma_call0].
 subst h_call0.
 store_valid.
-try rename h_tree_x2s2_5642 into h_tree_rx2s2x_560x.
-try rename H_tree_x2s2_5642 into H_tree_rx2s2x_560x.
-ssl_call_pre (h_tree_rx2s2x_560x).
+try rename h_tree_x2s2_52 into h_tree_rx1s2x_1x.
+try rename H_tree_x2s2_52 into H_tree_rx1s2x_1x.
+ssl_call_pre (h_tree_rx1s2x_1x).
 ssl_call (s2x).
-exists (h_tree_rx2s2x_560x);
+exists (h_tree_rx1s2x_1x);
 sslauto.
 ssl_frame_unfold.
 move=>h_call1.
