benchmarks/standard/tree/tree_size.v
@@ -8,6 +8,7 @@ From SSL
 Require Import core.
 From Hammer Require Import Hammer.
 (* Configure Hammer *)
+Set Hammer ATPLimit 60.
 Unset Hammer Eprover.
 Unset Hammer Vampire.
 Add Search Blacklist "fcsl.".
@@ -25,10 +26,10 @@ Add Search Blacklist "mathcomp.ssreflect.tuple".
 
 Require Import common.
 
-Lemma pure34 : (0) = (0). intros; hammer. Qed.
-Hint Resolve pure34: ssl_pure.
-Lemma pure35 (n1x2 : nat) (n2x2 : nat) : (0) <= (((1) + (n1x2)) + (n2x2)) -> (0) <= (n2x2) -> (0) <= (n1x2) -> (((1) + (n1x2)) + (n2x2)) = (((1) + (n1x2)) + (n2x2)). intros; hammer. Qed.
-Hint Resolve pure35: ssl_pure.
+Lemma pure1 : (0) = (0). intros; hammer. Qed.
+Hint Resolve pure1: ssl_pure.
+Lemma pure2 (n1x1 : nat) (n2x1 : nat) : (0) <= (((1) + (n1x1)) + (n2x1)) -> (0) <= (n1x1) -> (0) <= (n2x1) -> (((1) + (n1x1)) + (n2x1)) = (((1) + (n1x1)) + (n2x1)). intros; hammer. Qed.
+Hint Resolve pure2: ssl_pure.
 
 Definition tree_size_type :=
   forall (vprogs : ptr * ptr),
@@ -38,12 +39,12 @@ Definition tree_size_type :=
       let: (x, r) := vprogs in
       let: (n) := vghosts in
       exists h_treeN_xn_a,
-      (0) <= (n) /\ h = r :-> 0 \+ h_treeN_xn_a /\ treeN x n h_treeN_xn_a,
+      (0) <= (n) /\ h = r :-> (0) \+ h_treeN_xn_a /\ treeN x n h_treeN_xn_a,
     [vfun (_: unit) h =>
       let: (x, r) := vprogs in
       let: (n) := vghosts in
       exists h_treeN_xn_a,
-      h = r :-> n \+ h_treeN_xn_a /\ treeN x n h_treeN_xn_a
+      h = r :-> (n) \+ h_treeN_xn_a /\ treeN x n h_treeN_xn_a
     ]).
 
 Program Definition tree_size : tree_size_type :=
@@ -54,15 +55,15 @@ Program Definition tree_size : tree_size_type :=
       then
         ret tt
       else
-        vx2 <-- @read ptr x;
-        lx2 <-- @read ptr (x .+ 1);
-        rx2 <-- @read ptr (x .+ 2);
-        tree_size (lx2, r);;
-        n1x2 <-- @read nat r;
+        vx1 <-- @read ptr x;
+        lx1 <-- @read ptr (x .+ 1);
+        rx1 <-- @read ptr (x .+ 2);
+        tree_size (lx1, r);;
+        n1x1 <-- @read nat r;
         r ::= 0;;
-        tree_size (rx2, r);;
-        n2x2 <-- @read nat r;
-        r ::= ((1) + (n1x2)) + (n2x2);;
+        tree_size (rx1, r);;
+        n2x1 <-- @read nat r;
+        r ::= ((1) + (n1x1)) + (n2x1);;
         ret tt
     )).
 Obligation Tactic := intro; move=>[x r]; ssl_program_simpl.
@@ -87,73 +88,73 @@ sslauto.
 ssl_close 1;
 sslauto.
 ex_elim n1x n2x lx rx vx.
-ex_elim h_treeN_lxn1x_551x h_treeN_rxn2x_552x.
+ex_elim h_treeN_lxn1x_2x h_treeN_rxn2x_3x.
 move=>[phi_treeN_xn_a0] [phi_treeN_xn_a1] [phi_treeN_xn_a2].
 move=>[sigma_treeN_xn_a].
 subst h_treeN_xn_a.
-move=>[H_treeN_lxn1x_551x H_treeN_rxn2x_552x].
+move=>[H_treeN_lxn1x_2x H_treeN_rxn2x_3x].
 try rename h_treeN_xn_a into h_treeN_xn1xn2x_a.
 try rename H_treeN_xn_a into H_treeN_xn1xn2x_a.
 ssl_read x.
-try rename vx into vx2.
+try rename vx into vx1.
 ssl_read (x .+ 1).
-try rename lx into lx2.
-try rename h_treeN_lxn1x_551x into h_treeN_lx2n1x_551x.
-try rename H_treeN_lxn1x_551x into H_treeN_lx2n1x_551x.
+try rename lx into lx1.
+try rename h_treeN_lxn1x_2x into h_treeN_lx1n1x_2x.
+try rename H_treeN_lxn1x_2x into H_treeN_lx1n1x_2x.
 ssl_read (x .+ 2).
-try rename rx into rx2.
-try rename h_treeN_rxn2x_552x into h_treeN_rx2n2x_552x.
-try rename H_treeN_rxn2x_552x into H_treeN_rx2n2x_552x.
-try rename h_treeN_x1n1_a1 into h_treeN_lx2n1x_551x.
-try rename H_treeN_x1n1_a1 into H_treeN_lx2n1x_551x.
-ssl_call_pre (r :-> 0 \+ h_treeN_lx2n1x_551x).
+try rename rx into rx1.
+try rename h_treeN_rxn2x_3x into h_treeN_rx1n2x_3x.
+try rename H_treeN_rxn2x_3x into H_treeN_rx1n2x_3x.
+try rename h_treeN_x1n1_a1 into h_treeN_lx1n1x_2x.
+try rename H_treeN_x1n1_a1 into H_treeN_lx1n1x_2x.
+ssl_call_pre (r :-> (0) \+ h_treeN_lx1n1x_2x).
 ssl_call (n1x).
-exists (h_treeN_lx2n1x_551x);
+exists (h_treeN_lx1n1x_2x);
 sslauto.
 ssl_frame_unfold.
 move=>h_call0.
-ex_elim h_treeN_lx2n1x_551x.
+ex_elim h_treeN_lx1n1x_2x.
 move=>[sigma_call0].
 subst h_call0.
-move=>H_treeN_lx2n1x_551x.
+move=>H_treeN_lx1n1x_2x.
 store_valid.
 ssl_read r.
-try rename n1x into n1x2.
-try rename h_treeN_lx2n1x_551x into h_treeN_lx2n1x2_551x.
-try rename H_treeN_lx2n1x_551x into H_treeN_lx2n1x2_551x.
-try rename h_treeN_xn1xn2x_a into h_treeN_xn1x2n2x_a.
-try rename H_treeN_xn1xn2x_a into H_treeN_xn1x2n2x_a.
-try rename h_treeN_x2n2_a2 into h_treeN_rx2n2x_552x.
-try rename H_treeN_x2n2_a2 into H_treeN_rx2n2x_552x.
+try rename n1x into n1x1.
+try rename h_treeN_lx1n1x_2x into h_treeN_lx1n1x1_2x.
+try rename H_treeN_lx1n1x_2x into H_treeN_lx1n1x1_2x.
+try rename h_treeN_xn1xn2x_a into h_treeN_xn1x1n2x_a.
+try rename H_treeN_xn1xn2x_a into H_treeN_xn1x1n2x_a.
+try rename h_treeN_x2n2_a2 into h_treeN_rx1n2x_3x.
+try rename H_treeN_x2n2_a2 into H_treeN_rx1n2x_3x.
 ssl_write r.
-ssl_call_pre (r :-> 0 \+ h_treeN_rx2n2x_552x).
+ssl_call_pre (r :-> (0) \+ h_treeN_rx1n2x_3x).
 ssl_call (n2x).
-exists (h_treeN_rx2n2x_552x);
+exists (h_treeN_rx1n2x_3x);
 sslauto.
 ssl_frame_unfold.
 move=>h_call1.
-ex_elim h_treeN_rx2n2x_552x.
+ex_elim h_treeN_rx1n2x_3x.
 move=>[sigma_call1].
 subst h_call1.
-move=>H_treeN_rx2n2x_552x.
+move=>H_treeN_rx1n2x_3x.
 store_valid.
 ssl_read r.
-try rename n2x into n2x2.
-try rename h_treeN_rx2n2x_552x into h_treeN_rx2n2x2_552x.
-try rename H_treeN_rx2n2x_552x into H_treeN_rx2n2x2_552x.
-try rename h_treeN_xn1x2n2x_a into h_treeN_xn1x2n2x2_a.
-try rename H_treeN_xn1x2n2x_a into H_treeN_xn1x2n2x2_a.
-try rename h_treeN_lx1n11x_551x1 into h_treeN_lx2n1x2_551x.
-try rename H_treeN_lx1n11x_551x1 into H_treeN_lx2n1x2_551x.
-try rename h_treeN_r3xn21x_552x1 into h_treeN_rx2n2x2_552x.
-try rename H_treeN_r3xn21x_552x1 into H_treeN_rx2n2x2_552x.
+try rename n2x into n2x1.
+try rename h_treeN_xn1x1n2x_a into h_treeN_xn1x1n2x1_a.
+try rename H_treeN_xn1x1n2x_a into H_treeN_xn1x1n2x1_a.
+try rename h_treeN_rx1n2x_3x into h_treeN_rx1n2x1_3x.
+try rename H_treeN_rx1n2x_3x into H_treeN_rx1n2x1_3x.
+try rename h_treeN_lx2n11x_2x1 into h_treeN_lx1n1x1_2x.
+try rename H_treeN_lx2n11x_2x1 into H_treeN_lx1n1x1_2x.
+try rename h_treeN_r3xn21x_3x1 into h_treeN_rx1n2x1_3x.
+try rename H_treeN_r3xn21x_3x1 into H_treeN_rx1n2x1_3x.
 ssl_write r.
 ssl_write_post r.
 ssl_emp;
-exists (x :-> vx2 \+ x .+ 1 :-> lx2 \+ x .+ 2 :-> rx2 \+ h_treeN_lx2n1x2_551x \+ h_treeN_rx2n2x2_552x);
+exists (x :-> (vx1) \+ x .+ 1 :-> (lx1) \+ x .+ 2 :-> (rx1) \+ h_treeN_lx1n1x1_2x \+ h_treeN_rx1n2x1_3x);
 sslauto.
 ssl_close 2;
-exists (n1x2), (n2x2), (lx2), (rx2), (vx2), (h_treeN_lx2n1x2_551x), (h_treeN_rx2n2x2_552x);
+exists (n1x1), (n2x1), (lx1), (rx1), (vx1), (h_treeN_lx1n1x1_2x), (h_treeN_rx1n2x1_3x);
 sslauto.
 ssl_frame_unfold.
 ssl_frame_unfold.
